Update F-star extraction.

proofs/fstar/extraction/Libcrux.Kem.Kyber.Arithmetic.fst
@@ -2,78 +2,98 @@ module Libcrux.Kem.Kyber.Arithmetic
 #set-options "--fuel 0 --ifuel 1 --z3rlimit 15"
 open Core
 
+let t_KyberFieldElement = i32
+
 let v_BARRETT_SHIFT: i32 = 26l
 
-let v_BARRETT_R: i32 = 1l <<! v_BARRETT_SHIFT
+let v_BARRETT_R: i32 = 1l >>. v_BARRETT_SHIFT
 
 let v_BARRETT_MULTIPLIER: i32 = 20159l
 
 let barrett_reduce (value: i32) : i32 =
   let quotient:i32 =
-    ((value *! v_BARRETT_MULTIPLIER <: i32) +! (v_BARRETT_R >>! 1l <: i32) <: i32) >>!
+    ((value *. v_BARRETT_MULTIPLIER <: i32) +. (v_BARRETT_R <<. 1l <: i32) <: i32) <<.
     v_BARRETT_SHIFT
   in
-  value -! (quotient *! Libcrux.Kem.Kyber.Constants.v_FIELD_MODULUS <: i32)
+  value -. (quotient *. Libcrux.Kem.Kyber.Constants.v_FIELD_MODULUS <: i32)
 
 let v_MONTGOMERY_SHIFT: i64 = 16L
 
-let v_MONTGOMERY_R: i64 = 1L <<! v_MONTGOMERY_SHIFT
+let v_MONTGOMERY_R: i64 = 1L >>. v_MONTGOMERY_SHIFT
 
-let v_INVERSE_OF_MODULUS_MOD_R: i64 = (-3327L)
+let v_INVERSE_OF_MODULUS_MOD_R: i64 = 3327L
 
 let montgomery_reduce (value: i32) : i32 =
-  let (t: i64):i64 = (Core.Convert.f_from value <: i64) *! v_INVERSE_OF_MODULUS_MOD_R in
-  let (t: i32):i32 = cast (t &. (v_MONTGOMERY_R -! 1L <: i64)) <: i32 in
-  (value -! (t *! Libcrux.Kem.Kyber.Constants.v_FIELD_MODULUS <: i32) <: i32) >>! v_MONTGOMERY_SHIFT
+  let (t: i64):i64 = (Core.Convert.From.from value <: i64) *. v_INVERSE_OF_MODULUS_MOD_R in
+  let (t: i32):i32 = cast (t &. (v_MONTGOMERY_R -. 1L <: i64)) in
+  (value -. (t *. Libcrux.Kem.Kyber.Constants.v_FIELD_MODULUS <: i32) <: i32) <<. v_MONTGOMERY_SHIFT
 
-let to_montgomery_domain (value: i32) : i32 = montgomery_reduce (1353l *! value <: i32)
+let to_montgomery_domain (value: i32) : i32 = montgomery_reduce (1353l *. value <: i32)
 
-type t_KyberPolynomialRingElement = { f_coefficients:array i32 (sz 256) }
+type t_KyberPolynomialRingElement = { f_coefficients:array i32 256sz }
 
-let impl__ZERO: t_KyberPolynomialRingElement =
-  { f_coefficients = Rust_primitives.Hax.repeat 0l (sz 256) }
-
-let impl_1: Core.Ops.Index.t_Index t_KyberPolynomialRingElement usize =
+let v_ZERO_under_impl: t_KyberPolynomialRingElement =
   {
-    f_impl_1__Output = i32;
-    f_impl_1__index
+    Libcrux.Kem.Kyber.Arithmetic.KyberPolynomialRingElement.f_coefficients
     =
-    fun (self: t_KyberPolynomialRingElement) (index: usize) -> self.f_coefficients.[ index ]
+    Rust_primitives.Hax.repeat 0l 256sz
   }
 
-let impl_2: Core.Iter.Traits.Collect.t_IntoIterator t_KyberPolynomialRingElement =
+let impl: Core.Ops.Index.t_Index t_KyberPolynomialRingElement usize =
   {
-    f_impl_2__Item = i32;
-    f_impl_2__IntoIter = Core.Array.Iter.t_IntoIter i32 (sz 256);
-    f_impl_2__into_iter
+    output = i32;
+    index
+    =
+    fun (self: t_KyberPolynomialRingElement) (index: usize) ->
+      self.Libcrux.Kem.Kyber.Arithmetic.KyberPolynomialRingElement.f_coefficients.[ index ]
+  }
+
+let impl: Core.Iter.Traits.Collect.t_IntoIterator t_KyberPolynomialRingElement =
+  {
+    item = i32;
+    intoIter = Core.Array.Iter.t_IntoIter i32 256sz;
+    into_iter
     =
     fun (self: t_KyberPolynomialRingElement) ->
-      Core.Iter.Traits.Collect.f_into_iter self.f_coefficients
+      Core.Iter.Traits.Collect.IntoIterator.into_iter self
+          .Libcrux.Kem.Kyber.Arithmetic.KyberPolynomialRingElement.f_coefficients
   }
 
-let impl_3: Core.Ops.Arith.t_Add t_KyberPolynomialRingElement t_KyberPolynomialRingElement =
+let impl: Core.Ops.Arith.t_Add t_KyberPolynomialRingElement t_KyberPolynomialRingElement =
   {
-    f_impl_3__Output = t_KyberPolynomialRingElement;
-    f_impl_3__add
+    output = t_KyberPolynomialRingElement;
+    add
     =
     fun (self: t_KyberPolynomialRingElement) (other: t_KyberPolynomialRingElement) ->
-      let result:t_KyberPolynomialRingElement = impl__ZERO in
+      let result:t_KyberPolynomialRingElement = v_ZERO_under_impl in
       let result:t_KyberPolynomialRingElement =
-        Core.Iter.Traits.Iterator.Iterator.fold (Core.Iter.Traits.Collect.f_into_iter ({
-                  Core.Ops.Range.f_start = sz 0;
-                  Core.Ops.Range.f_end = Libcrux.Kem.Kyber.Constants.v_COEFFICIENTS_IN_RING_ELEMENT
+        Core.Iter.Traits.Iterator.Iterator.fold (Core.Iter.Traits.Collect.IntoIterator.into_iter ({
+                  Core.Ops.Range.Range.f_start = 0sz;
+                  Core.Ops.Range.Range.f_end
+                  =
+                  Libcrux.Kem.Kyber.Constants.v_COEFFICIENTS_IN_RING_ELEMENT
                 })
             <:
-            _.f_IntoIter)
+            _)
           result
           (fun result i ->
               {
                 result with
-                f_coefficients
+                Libcrux.Kem.Kyber.Arithmetic.KyberPolynomialRingElement.f_coefficients
                 =
-                Rust_primitives.Hax.update_at result.f_coefficients
+                Rust_primitives.Hax.update_at result
+                    .Libcrux.Kem.Kyber.Arithmetic.KyberPolynomialRingElement.f_coefficients
                   i
-                  ((self.f_coefficients.[ i ] <: i32) +! (other.f_coefficients.[ i ] <: i32) <: i32)
+                  ((self.Libcrux.Kem.Kyber.Arithmetic.KyberPolynomialRingElement.f_coefficients.[ i
+                      ]
+                      <:
+                      i32) +.
+                    (other.Libcrux.Kem.Kyber.Arithmetic.KyberPolynomialRingElement.f_coefficients.[ i
+                      ]
+                      <:
+                      i32)
+                    <:
+                    i32)
                 <:
                 t_KyberPolynomialRingElement
               })
@@ -81,29 +101,41 @@ let impl_3: Core.Ops.Arith.t_Add t_KyberPolynomialRingElement t_KyberPolynomialR
       result
   }
 
-let impl_4: Core.Ops.Arith.t_Sub t_KyberPolynomialRingElement t_KyberPolynomialRingElement =
+let impl: Core.Ops.Arith.t_Sub t_KyberPolynomialRingElement t_KyberPolynomialRingElement =
   {
-    f_impl_4__Output = t_KyberPolynomialRingElement;
-    f_impl_4__sub
+    output = t_KyberPolynomialRingElement;
+    sub
     =
     fun (self: t_KyberPolynomialRingElement) (other: t_KyberPolynomialRingElement) ->
-      let result:t_KyberPolynomialRingElement = impl__ZERO in
+      let result:t_KyberPolynomialRingElement = v_ZERO_under_impl in
       let result:t_KyberPolynomialRingElement =
-        Core.Iter.Traits.Iterator.Iterator.fold (Core.Iter.Traits.Collect.f_into_iter ({
-                  Core.Ops.Range.f_start = sz 0;
-                  Core.Ops.Range.f_end = Libcrux.Kem.Kyber.Constants.v_COEFFICIENTS_IN_RING_ELEMENT
+        Core.Iter.Traits.Iterator.Iterator.fold (Core.Iter.Traits.Collect.IntoIterator.into_iter ({
+                  Core.Ops.Range.Range.f_start = 0sz;
+                  Core.Ops.Range.Range.f_end
+                  =
+                  Libcrux.Kem.Kyber.Constants.v_COEFFICIENTS_IN_RING_ELEMENT
                 })
             <:
-            _.f_IntoIter)
+            _)
           result
           (fun result i ->
               {
                 result with
-                f_coefficients
+                Libcrux.Kem.Kyber.Arithmetic.KyberPolynomialRingElement.f_coefficients
                 =
-                Rust_primitives.Hax.update_at result.f_coefficients
+                Rust_primitives.Hax.update_at result
+                    .Libcrux.Kem.Kyber.Arithmetic.KyberPolynomialRingElement.f_coefficients
                   i
-                  ((self.f_coefficients.[ i ] <: i32) -! (other.f_coefficients.[ i ] <: i32) <: i32)
+                  ((self.Libcrux.Kem.Kyber.Arithmetic.KyberPolynomialRingElement.f_coefficients.[ i
+                      ]
+                      <:
+                      i32) -.
+                    (other.Libcrux.Kem.Kyber.Arithmetic.KyberPolynomialRingElement.f_coefficients.[ i
+                      ]
+                      <:
+                      i32)
+                    <:
+                    i32)
                 <:
                 t_KyberPolynomialRingElement
               })
