proofs/fstar/extraction/Libcrux.Kem.Kyber.Ind_cpa.fst
@@ -2,103 +2,120 @@ module Libcrux.Kem.Kyber.Ind_cpa
 #set-options "--fuel 0 --ifuel 1 --z3rlimit 15"
 open Core
 
-type t_PrivateKey (#v_SIZE: usize) = { f_value:array u8 v_SIZE }
+type t_PrivateKey = { f_value:array u8 v_SIZE }
 
-let impl (#v_SIZE: usize) : Core.Convert.t_AsRef (t_PrivateKey v_SIZE) (slice u8) =
+let impl (#size: usize) : Core.Convert.t_AsRef (t_PrivateKey v_SIZE) (slice u8) =
   {
-    f_impl__as_ref
+    as_ref
     =
-    fun (#v_SIZE: usize) (self: t_PrivateKey v_SIZE) -> Rust_primitives.unsize self.f_value
+    fun (#size: usize) (self: t_PrivateKey v_SIZE) ->
+      Rust_primitives.unsize self.Libcrux.Kem.Kyber.Ind_cpa.PrivateKey.f_value
   }
 
-let impl_1 (#v_SIZE: usize) : Core.Convert.t_From (t_PrivateKey v_SIZE) (array u8 v_SIZE) =
-  { f_impl_1__from = fun (#v_SIZE: usize) (value: array u8 v_SIZE) -> { f_value = value } }
-
-let impl_2 (#v_SIZE: usize) : Core.Convert.t_From (array u8 v_SIZE) (t_PrivateKey v_SIZE) =
-  { f_impl_2__from = fun (#v_SIZE: usize) (value: t_PrivateKey v_SIZE) -> value.f_value }
-
-let impl_3 (#v_SIZE: usize) : Core.Convert.t_TryFrom (t_PrivateKey v_SIZE) (slice u8) =
+let impl (#size: usize) : Core.Convert.t_From (t_PrivateKey v_SIZE) (array u8 v_SIZE) =
   {
-    f_impl_3__Error = Core.Array.t_TryFromSliceError;
-    f_impl_3__try_from
+    from
     =
-    fun (#v_SIZE: usize) (value: slice u8) ->
+    fun (#size: usize) (value: array u8 v_SIZE) ->
+      { Libcrux.Kem.Kyber.Ind_cpa.PrivateKey.f_value = value }
+  }
+
+let impl (#size: usize) : Core.Convert.t_From (array u8 v_SIZE) (t_PrivateKey v_SIZE) =
+  {
+    from
+    =
+    fun (#size: usize) (value: t_PrivateKey v_SIZE) ->
+      value.Libcrux.Kem.Kyber.Ind_cpa.PrivateKey.f_value
+  }
+
+let impl (#size: usize) : Core.Convert.t_TryFrom (t_PrivateKey v_SIZE) (slice u8) =
+  {
+    error = Core.Array.t_TryFromSliceError;
+    try_from
+    =
+    fun (#size: usize) (value: slice u8) ->
       Rust_primitives.Hax.Control_flow_monad.Mexception.run (let* hoist2:array u8 v_SIZE =
             match
-              Core.Ops.Try_trait.f_branch (Core.Convert.f_try_into value
+              Core.Ops.Try_trait.Try.branch (Core.Convert.TryInto.try_into value
                   <:
-                  Core.Result.t_Result (array u8 v_SIZE) _.f_Error)
+                  Core.Result.t_Result (array u8 v_SIZE) _)
             with
-            | Core.Ops.Control_flow.ControlFlow_Break
-              { Core.Ops.Control_flow.ControlFlow._0 = residual } ->
+            | Core.Ops.Control_flow.ControlFlow_Break residual ->
               let* hoist1:Rust_primitives.Hax.t_Never =
-                Core.Ops.Control_flow.ControlFlow.v_Break (Core.Ops.Try_trait.f_from_residual residual
-
+                Core.Ops.Control_flow.ControlFlow.v_Break (Core.Ops.Try_trait.FromResidual.from_residual
+                      residual
                     <:
                     Core.Result.t_Result (t_PrivateKey v_SIZE) Core.Array.t_TryFromSliceError)
               in
               Core.Ops.Control_flow.ControlFlow_Continue (Rust_primitives.Hax.never_to_any hoist1)
-            | Core.Ops.Control_flow.ControlFlow_Continue
-              { Core.Ops.Control_flow.ControlFlow._0 = v_val } ->
+            | Core.Ops.Control_flow.ControlFlow_Continue v_val ->
               Core.Ops.Control_flow.ControlFlow_Continue v_val
           in
           Core.Ops.Control_flow.ControlFlow_Continue
-          (let hoist3:t_PrivateKey v_SIZE = { f_value = hoist2 } in
+          (let hoist3:t_PrivateKey v_SIZE =
+              { Libcrux.Kem.Kyber.Ind_cpa.PrivateKey.f_value = hoist2 }
+            in
             Core.Result.Result_Ok hoist3))
   }
 
-let impl_4 (#v_SIZE: usize) : Core.Ops.Index.t_Index (t_PrivateKey v_SIZE) usize =
+let impl (#size: usize) : Core.Ops.Index.t_Index (t_PrivateKey v_SIZE) usize =
   {
-    f_impl_4__Output = u8;
-    f_impl_4__index
+    output = u8;
+    index
     =
-    fun (#v_SIZE: usize) (self: t_PrivateKey v_SIZE) (index: usize) -> self.f_value.[ index ]
+    fun (#size: usize) (self: t_PrivateKey v_SIZE) (index: usize) ->
+      self.Libcrux.Kem.Kyber.Ind_cpa.PrivateKey.f_value.[ index ]
   }
 
-let impl_5 (#v_SIZE: usize)
+let impl (#size: usize)
     : Core.Ops.Index.t_Index (t_PrivateKey v_SIZE) (Core.Ops.Range.t_Range usize) =
   {
-    f_impl_5__Output = slice u8;
-    f_impl_5__index
+    output = slice u8;
+    index
     =
-    fun (#v_SIZE: usize) (self: t_PrivateKey v_SIZE) (range: Core.Ops.Range.t_Range usize) ->
-      self.f_value.[ range ]
+    fun (#size: usize) (self: t_PrivateKey v_SIZE) (range: Core.Ops.Range.t_Range usize) ->
+      self.Libcrux.Kem.Kyber.Ind_cpa.PrivateKey.f_value.[ range ]
   }
 
-let impl_6 (#v_SIZE: usize)
+let impl (#size: usize)
     : Core.Ops.Index.t_Index (t_PrivateKey v_SIZE) (Core.Ops.Range.t_RangeTo usize) =
   {
-    f_impl_6__Output = slice u8;
-    f_impl_6__index
+    output = slice u8;
+    index
     =
-    fun (#v_SIZE: usize) (self: t_PrivateKey v_SIZE) (range: Core.Ops.Range.t_RangeTo usize) ->
-      self.f_value.[ range ]
+    fun (#size: usize) (self: t_PrivateKey v_SIZE) (range: Core.Ops.Range.t_RangeTo usize) ->
+      self.Libcrux.Kem.Kyber.Ind_cpa.PrivateKey.f_value.[ range ]
   }
 
-let impl_7 (#v_SIZE: usize)
+let impl (#size: usize)
     : Core.Ops.Index.t_Index (t_PrivateKey v_SIZE) (Core.Ops.Range.t_RangeFrom usize) =
   {
-    f_impl_7__Output = slice u8;
-    f_impl_7__index
+    output = slice u8;
+    index
     =
-    fun (#v_SIZE: usize) (self: t_PrivateKey v_SIZE) (range: Core.Ops.Range.t_RangeFrom usize) ->
-      self.f_value.[ range ]
+    fun (#size: usize) (self: t_PrivateKey v_SIZE) (range: Core.Ops.Range.t_RangeFrom usize) ->
+      self.Libcrux.Kem.Kyber.Ind_cpa.PrivateKey.f_value.[ range ]
   }
 
-let impl_8__as_slice (#v_SIZE: usize) (self: t_PrivateKey v_SIZE) : array u8 v_SIZE = self.f_value
+let as_slice_under_impl_8 (#size: usize) (self: t_PrivateKey v_SIZE) : array u8 v_SIZE =
+  self.Libcrux.Kem.Kyber.Ind_cpa.PrivateKey.f_value
 
-let impl_8__split_at (#v_SIZE: usize) (self: t_PrivateKey v_SIZE) (mid: usize)
+let split_at_under_impl_8 (#size: usize) (self: t_PrivateKey v_SIZE) (mid: usize)
     : (slice u8 & slice u8) =
-  Core.Slice.impl__split_at (Rust_primitives.unsize self.f_value <: slice u8) mid
+  Core.Slice.split_at_under_impl (Rust_primitives.unsize self
+          .Libcrux.Kem.Kyber.Ind_cpa.PrivateKey.f_value
+      <:
+      slice u8)
+    mid
 
-let impl_8__len (#v_SIZE: usize) (self: t_PrivateKey v_SIZE) : usize = v_SIZE
+let len_under_impl_8 (#size: usize) (self: t_PrivateKey v_SIZE) : usize = v_SIZE
 
-let sample_matrix_A (#v_K: usize) (seed: array u8 (sz 34)) (transpose: bool)
+let sample_matrix_A (#k: usize) (seed: array u8 34sz) (transpose: bool)
     : (array (array Libcrux.Kem.Kyber.Arithmetic.t_KyberPolynomialRingElement v_K) v_K &
       Core.Option.t_Option Libcrux.Kem.Kyber.t_BadRejectionSamplingRandomnessError) =
   let v_A_transpose:array (array Libcrux.Kem.Kyber.Arithmetic.t_KyberPolynomialRingElement v_K) v_K
   =
-    Rust_primitives.Hax.repeat (Rust_primitives.Hax.repeat Libcrux.Kem.Kyber.Arithmetic.impl__ZERO
+    Rust_primitives.Hax.repeat (Rust_primitives.Hax.repeat Libcrux.Kem.Kyber.Arithmetic.v_ZERO_under_impl
           v_K
         <:
         array Libcrux.Kem.Kyber.Arithmetic.t_KyberPolynomialRingElement v_K)
@@ -111,64 +128,58 @@ let sample_matrix_A (#v_K: usize) (seed: array u8 (sz 34)) (transpose: bool)
   let v_A_transpose, sampling_A_error:(array
       (array Libcrux.Kem.Kyber.Arithmetic.t_KyberPolynomialRingElement v_K) v_K &
     Core.Option.t_Option Libcrux.Kem.Kyber.t_BadRejectionSamplingRandomnessError) =
-    Core.Iter.Traits.Iterator.Iterator.fold (Core.Iter.Traits.Collect.f_into_iter ({
-              Core.Ops.Range.f_start = sz 0;
-              Core.Ops.Range.f_end = v_K
+    Core.Iter.Traits.Iterator.Iterator.fold (Core.Iter.Traits.Collect.IntoIterator.into_iter ({
+              Core.Ops.Range.Range.f_start = 0sz;
+              Core.Ops.Range.Range.f_end = v_K
             })
         <:
-        _.f_IntoIter)
+        _)
       (v_A_transpose, sampling_A_error)
       (fun (v_A_transpose, sampling_A_error) i ->
-          let seeds:array (array u8 (sz 34)) v_K = Rust_primitives.Hax.repeat seed v_K in
-          let seeds:array (array u8 (sz 34)) v_K =
-            Core.Iter.Traits.Iterator.Iterator.fold (Core.Iter.Traits.Collect.f_into_iter ({
-                      Core.Ops.Range.f_start = sz 0;
-                      Core.Ops.Range.f_end = v_K
-                    })
+          let seeds:array (array u8 34sz) v_K = Rust_primitives.Hax.repeat seed v_K in
+          let seeds:array (array u8 34sz) v_K =
+            Core.Iter.Traits.Iterator.Iterator.fold (Core.Iter.Traits.Collect.IntoIterator.into_iter
+                  ({ Core.Ops.Range.Range.f_start = 0sz; Core.Ops.Range.Range.f_end = v_K })
                 <:
-                _.f_IntoIter)
+                _)
               seeds
               (fun seeds j ->
-                  let seeds:array (array u8 (sz 34)) v_K =
+                  let seeds:array (array u8 34sz) v_K =
                     Rust_primitives.Hax.update_at seeds
                       j
-                      (Rust_primitives.Hax.update_at (seeds.[ j ] <: array u8 (sz 34))
-                          (sz 32)
-                          (cast i <: u8)
+                      (Rust_primitives.Hax.update_at (seeds.[ j ] <: array u8 34sz) 32sz (cast i)
                         <:
-                        array u8 (sz 34))
+                        array u8 34sz)
                   in
-                  let seeds:array (array u8 (sz 34)) v_K =
+                  let seeds:array (array u8 34sz) v_K =
                     Rust_primitives.Hax.update_at seeds
                       j
-                      (Rust_primitives.Hax.update_at (seeds.[ j ] <: array u8 (sz 34))
-                          (sz 33)
-                          (cast j <: u8)
+                      (Rust_primitives.Hax.update_at (seeds.[ j ] <: array u8 34sz) 33sz (cast j)
                         <:
-                        array u8 (sz 34))
+                        array u8 34sz)
                   in
                   seeds)
           in
-          let xof_bytes:array (array u8 (sz 840)) v_K =
+          let xof_bytes:array (array u8 840sz) v_K =
             Libcrux.Kem.Kyber.Hash_functions.v_XOFx4 seeds
           in
-          Core.Iter.Traits.Iterator.Iterator.fold (Core.Iter.Traits.Collect.f_into_iter ({
-                    Core.Ops.Range.f_start = sz 0;
-                    Core.Ops.Range.f_end = v_K
+          Core.Iter.Traits.Iterator.Iterator.fold (Core.Iter.Traits.Collect.IntoIterator.into_iter ({
+                    Core.Ops.Range.Range.f_start = 0sz;
+                    Core.Ops.Range.Range.f_end = v_K
                   })
               <:
-              _.f_IntoIter)
+              _)
             (v_A_transpose, sampling_A_error)
             (fun (v_A_transpose, sampling_A_error) j ->
                 let sampled, error:(Libcrux.Kem.Kyber.Arithmetic.t_KyberPolynomialRingElement &
                   Core.Option.t_Option Libcrux.Kem.Kyber.t_BadRejectionSamplingRandomnessError) =
                   Libcrux.Kem.Kyber.Sampling.sample_from_uniform_distribution (xof_bytes.[ j ]
                       <:
-                      array u8 (sz 840))
+                      array u8 840sz)
                 in
                 let sampling_A_error:Core.Option.t_Option
                 Libcrux.Kem.Kyber.t_BadRejectionSamplingRandomnessError =
-                  if Core.Option.impl__is_some error
+                  if Core.Option.is_some_under_impl error
                   then
                     let sampling_A_error:Core.Option.t_Option
                     Libcrux.Kem.Kyber.t_BadRejectionSamplingRandomnessError =
@@ -209,31 +220,34 @@ let sample_matrix_A (#v_K: usize) (seed: array u8 (sz 34)) (transpose: bool)
   in
   v_A_transpose, sampling_A_error
 
-let cbd (#v_K: usize) (prf_input: array u8 (sz 33))
+let cbd (#k #eta #eta_randomness_size: usize) (prf_input: array u8 33sz)
     : (array Libcrux.Kem.Kyber.Arithmetic.t_KyberPolynomialRingElement v_K & u8) =
   let domain_separator:u8 = 0uy in
   let re_as_ntt:array Libcrux.Kem.Kyber.Arithmetic.t_KyberPolynomialRingElement v_K =
-    Rust_primitives.Hax.repeat Libcrux.Kem.Kyber.Arithmetic.impl__ZERO v_K
+    Rust_primitives.Hax.repeat Libcrux.Kem.Kyber.Arithmetic.v_ZERO_under_impl v_K
   in
-  let domain_separator, prf_input, re_as_ntt:(Prims.unit & array u8 (sz 33) &
+  let domain_separator, prf_input, re_as_ntt:(Prims.unit & array u8 33sz &
     array Libcrux.Kem.Kyber.Arithmetic.t_KyberPolynomialRingElement v_K) =
-    Core.Iter.Traits.Iterator.Iterator.fold (Core.Iter.Traits.Collect.f_into_iter ({
-              Core.Ops.Range.f_start = sz 0;
-              Core.Ops.Range.f_end = v_K
+    Core.Iter.Traits.Iterator.Iterator.fold (Core.Iter.Traits.Collect.IntoIterator.into_iter ({
+              Core.Ops.Range.Range.f_start = 0sz;
+              Core.Ops.Range.Range.f_end = v_K
             })
         <:
-        _.f_IntoIter)
+        _)
       (domain_separator, prf_input, re_as_ntt)
       (fun (domain_separator, prf_input, re_as_ntt) i ->
-          let prf_input:array u8 (sz 33) =
-            Rust_primitives.Hax.update_at prf_input (sz 32) domain_separator
+          let prf_input:array u8 33sz =
+            Rust_primitives.Hax.update_at prf_input 32sz domain_separator
           in
-          let domain_separator:Prims.unit = domain_separator +! 1uy in
-          let (prf_output: array u8 (sz 128)):array u8 (sz 128) =
+          let domain_separator:Prims.unit = domain_separator +. 1uy in
+          let (prf_output: array u8 v_ETA_RANDOMNESS_SIZE):array u8 v_ETA_RANDOMNESS_SIZE =
             Libcrux.Kem.Kyber.Hash_functions.v_PRF (Rust_primitives.unsize prf_input <: slice u8)
           in
           let r:Libcrux.Kem.Kyber.Arithmetic.t_KyberPolynomialRingElement =
-            Libcrux.Kem.Kyber.Sampling.sample_from_binomial_distribution_2_ prf_output
+            Libcrux.Kem.Kyber.Sampling.sample_from_binomial_distribution (Rust_primitives.unsize prf_output
+
+                <:
+                slice u8)
           in
           let re_as_ntt:array Libcrux.Kem.Kyber.Arithmetic.t_KyberPolynomialRingElement v_K =
             Rust_primitives.Hax.update_at re_as_ntt
@@ -247,40 +261,38 @@ let cbd (#v_K: usize) (prf_input: array u8 (sz 33))
   re_as_ntt, domain_separator
 
 let encode_12_
-      (#v_K #v_OUT_LEN: usize)
+      (#k #out_len: usize)
       (input: array Libcrux.Kem.Kyber.Arithmetic.t_KyberPolynomialRingElement v_K)
     : array u8 v_OUT_LEN =
   let out:array u8 v_OUT_LEN = Rust_primitives.Hax.repeat 0uy v_OUT_LEN in
   let out:array u8 v_OUT_LEN =
-    Core.Iter.Traits.Iterator.Iterator.fold (Core.Iter.Traits.Collect.f_into_iter (Core.Iter.Traits.Iterator.f_enumerate
-              (Core.Iter.Traits.Collect.f_into_iter input <: _.f_IntoIter)
+    Core.Iter.Traits.Iterator.Iterator.fold (Core.Iter.Traits.Collect.IntoIterator.into_iter (Core.Iter.Traits.Iterator.Iterator.enumerate
+              (Core.Iter.Traits.Collect.IntoIterator.into_iter input <: _)
             <:
             Core.Iter.Adapters.Enumerate.t_Enumerate
             (Core.Array.Iter.t_IntoIter Libcrux.Kem.Kyber.Arithmetic.t_KyberPolynomialRingElement
                 v_K))
         <:
-        _.f_IntoIter)
+        _)
       out
       (fun out (i, re) ->
           Rust_primitives.Hax.update_at out
             ({
-                Core.Ops.Range.f_start
+                Core.Ops.Range.Range.f_start
                 =
-                i *! Libcrux.Kem.Kyber.Constants.v_BYTES_PER_RING_ELEMENT <: usize;
-                Core.Ops.Range.f_end
+                i *. Libcrux.Kem.Kyber.Constants.v_BYTES_PER_RING_ELEMENT <: usize;
+                Core.Ops.Range.Range.f_end
                 =
-                (i +! sz 1 <: usize) *! Libcrux.Kem.Kyber.Constants.v_BYTES_PER_RING_ELEMENT
-                <:
-                usize
+                (i +. 1sz <: usize) *. Libcrux.Kem.Kyber.Constants.v_BYTES_PER_RING_ELEMENT <: usize
               })
-            (Core.Slice.impl__copy_from_slice (Core.Ops.Index.IndexMut.index_mut out
+            (Core.Slice.copy_from_slice_under_impl (Core.Ops.Index.IndexMut.index_mut out
                     ({
-                        Core.Ops.Range.f_start
+                        Core.Ops.Range.Range.f_start
                         =
-                        i *! Libcrux.Kem.Kyber.Constants.v_BYTES_PER_RING_ELEMENT <: usize;
-                        Core.Ops.Range.f_end
+                        i *. Libcrux.Kem.Kyber.Constants.v_BYTES_PER_RING_ELEMENT <: usize;
+                        Core.Ops.Range.Range.f_end
                         =
-                        (i +! sz 1 <: usize) *! Libcrux.Kem.Kyber.Constants.v_BYTES_PER_RING_ELEMENT
+                        (i +. 1sz <: usize) *. Libcrux.Kem.Kyber.Constants.v_BYTES_PER_RING_ELEMENT
                         <:
                         usize
                       })
@@ -288,7 +300,7 @@ let encode_12_
                   slice u8)
                 (Rust_primitives.unsize (Libcrux.Kem.Kyber.Serialize.serialize_little_endian re
                       <:
-                      array u8 (sz 384))
+                      array u8 384sz)
                   <:
                   slice u8)
               <:
@@ -299,38 +311,41 @@ let encode_12_
   out
 
 let generate_keypair
-      (#v_K #v_PRIVATE_KEY_SIZE #v_PUBLIC_KEY_SIZE #v_BYTES_PER_RING_ELEMENT: usize)
+      (#k #private_key_size #public_key_size #bytes_per_ring_element #eta1 #eta1_randomness_size:
+          usize)
       (key_generation_seed: slice u8)
     : ((t_PrivateKey v_PRIVATE_KEY_SIZE & Libcrux.Kem.Kyber.t_KyberPublicKey v_PUBLIC_KEY_SIZE) &
       Core.Option.t_Option Libcrux.Kem.Kyber.t_BadRejectionSamplingRandomnessError) =
-  let (prf_input: array u8 (sz 33)):array u8 (sz 33) = Rust_primitives.Hax.repeat 0uy (sz 33) in
+  let (prf_input: array u8 33sz):array u8 33sz = Rust_primitives.Hax.repeat 0uy 33sz in
   let secret_as_ntt:array Libcrux.Kem.Kyber.Arithmetic.t_KyberPolynomialRingElement v_K =
-    Rust_primitives.Hax.repeat Libcrux.Kem.Kyber.Arithmetic.impl__ZERO v_K
+    Rust_primitives.Hax.repeat Libcrux.Kem.Kyber.Arithmetic.v_ZERO_under_impl v_K
   in
   let error_as_ntt:array Libcrux.Kem.Kyber.Arithmetic.t_KyberPolynomialRingElement v_K =
-    Rust_primitives.Hax.repeat Libcrux.Kem.Kyber.Arithmetic.impl__ZERO v_K
+    Rust_primitives.Hax.repeat Libcrux.Kem.Kyber.Arithmetic.v_ZERO_under_impl v_K
   in
   let (domain_separator: u8):u8 = 0uy in
-  let hashed:array u8 (sz 64) = Libcrux.Kem.Kyber.Hash_functions.v_G key_generation_seed in
+  let hashed:array u8 64sz = Libcrux.Kem.Kyber.Hash_functions.v_G key_generation_seed in
   let seed_for_A, seed_for_secret_and_error:(slice u8 & slice u8) =
-    Core.Slice.impl__split_at (Rust_primitives.unsize hashed <: slice u8) (sz 32)
+    Core.Slice.split_at_under_impl (Rust_primitives.unsize hashed <: slice u8) 32sz
   in
   let v_A_transpose, sampling_A_error:(array
       (array Libcrux.Kem.Kyber.Arithmetic.t_KyberPolynomialRingElement v_K) v_K &
     Core.Option.t_Option Libcrux.Kem.Kyber.t_BadRejectionSamplingRandomnessError) =
-    sample_matrix_A (Libcrux.Kem.Kyber.Conversions.into_padded_array seed_for_A <: array u8 (sz 34))
+    sample_matrix_A (Libcrux.Kem.Kyber.Conversions.into_padded_array seed_for_A <: array u8 34sz)
       true
   in
-  let prf_input:array u8 (sz 33) =
+  let prf_input:array u8 33sz =
     Rust_primitives.Hax.update_at prf_input
       ({
-          Core.Ops.Range.f_start = sz 0;
-          Core.Ops.Range.f_end = Core.Slice.impl__len seed_for_secret_and_error <: usize
+          Core.Ops.Range.Range.f_start = 0sz;
+          Core.Ops.Range.Range.f_end = Core.Slice.len_under_impl seed_for_secret_and_error <: usize
         })
-      (Core.Slice.impl__copy_from_slice (Core.Ops.Index.IndexMut.index_mut prf_input
+      (Core.Slice.copy_from_slice_under_impl (Core.Ops.Index.IndexMut.index_mut prf_input
               ({
-                  Core.Ops.Range.f_start = sz 0;
-                  Core.Ops.Range.f_end = Core.Slice.impl__len seed_for_secret_and_error <: usize
+                  Core.Ops.Range.Range.f_start = 0sz;
+                  Core.Ops.Range.Range.f_end
+                  =
+                  Core.Slice.len_under_impl seed_for_secret_and_error <: usize
                 })
             <:
             slice u8)
@@ -338,25 +353,28 @@ let generate_keypair
         <:
         slice u8)
   in
-  let domain_separator, prf_input, secret_as_ntt:(Prims.unit & array u8 (sz 33) &
+  let domain_separator, prf_input, secret_as_ntt:(Prims.unit & array u8 33sz &
     array Libcrux.Kem.Kyber.Arithmetic.t_KyberPolynomialRingElement v_K) =
-    Core.Iter.Traits.Iterator.Iterator.fold (Core.Iter.Traits.Collect.f_into_iter ({
-              Core.Ops.Range.f_start = sz 0;
-              Core.Ops.Range.f_end = v_K
+    Core.Iter.Traits.Iterator.Iterator.fold (Core.Iter.Traits.Collect.IntoIterator.into_iter ({
+              Core.Ops.Range.Range.f_start = 0sz;
+              Core.Ops.Range.Range.f_end = v_K
             })
         <:
-        _.f_IntoIter)
+        _)
       (domain_separator, prf_input, secret_as_ntt)
       (fun (domain_separator, prf_input, secret_as_ntt) i ->
-          let prf_input:array u8 (sz 33) =
-            Rust_primitives.Hax.update_at prf_input (sz 32) domain_separator
+          let prf_input:array u8 33sz =
+            Rust_primitives.Hax.update_at prf_input 32sz domain_separator
           in
-          let domain_separator:Prims.unit = domain_separator +! 1uy in
-          let (prf_output: array u8 (sz 128)):array u8 (sz 128) =
+          let domain_separator:Prims.unit = domain_separator +. 1uy in
+          let (prf_output: array u8 v_ETA1_RANDOMNESS_SIZE):array u8 v_ETA1_RANDOMNESS_SIZE =
             Libcrux.Kem.Kyber.Hash_functions.v_PRF (Rust_primitives.unsize prf_input <: slice u8)
           in
           let secret:Libcrux.Kem.Kyber.Arithmetic.t_KyberPolynomialRingElement =
-            Libcrux.Kem.Kyber.Sampling.sample_from_binomial_distribution_2_ prf_output
+            Libcrux.Kem.Kyber.Sampling.sample_from_binomial_distribution (Rust_primitives.unsize prf_output
+
+                <:
+                slice u8)
           in
           let secret_as_ntt:array Libcrux.Kem.Kyber.Arithmetic.t_KyberPolynomialRingElement v_K =
             Rust_primitives.Hax.update_at secret_as_ntt
@@ -369,24 +387,27 @@ let generate_keypair
   in
   let domain_separator, error_as_ntt, prf_input:(Prims.unit &
     array Libcrux.Kem.Kyber.Arithmetic.t_KyberPolynomialRingElement v_K &
-    array u8 (sz 33)) =
-    Core.Iter.Traits.Iterator.Iterator.fold (Core.Iter.Traits.Collect.f_into_iter ({
-              Core.Ops.Range.f_start = sz 0;
-              Core.Ops.Range.f_end = v_K
+    array u8 33sz) =
+    Core.Iter.Traits.Iterator.Iterator.fold (Core.Iter.Traits.Collect.IntoIterator.into_iter ({
+              Core.Ops.Range.Range.f_start = 0sz;
+              Core.Ops.Range.Range.f_end = v_K
             })
         <:
-        _.f_IntoIter)
+        _)
       (domain_separator, error_as_ntt, prf_input)
       (fun (domain_separator, error_as_ntt, prf_input) i ->
-          let prf_input:array u8 (sz 33) =
-            Rust_primitives.Hax.update_at prf_input (sz 32) domain_separator
+          let prf_input:array u8 33sz =
+            Rust_primitives.Hax.update_at prf_input 32sz domain_separator
           in
-          let domain_separator:Prims.unit = domain_separator +! 1uy in
-          let (prf_output: array u8 (sz 128)):array u8 (sz 128) =
+          let domain_separator:Prims.unit = domain_separator +. 1uy in
+          let (prf_output: array u8 v_ETA1_RANDOMNESS_SIZE):array u8 v_ETA1_RANDOMNESS_SIZE =
             Libcrux.Kem.Kyber.Hash_functions.v_PRF (Rust_primitives.unsize prf_input <: slice u8)
           in
           let error:Libcrux.Kem.Kyber.Arithmetic.t_KyberPolynomialRingElement =
-            Libcrux.Kem.Kyber.Sampling.sample_from_binomial_distribution_2_ prf_output
+            Libcrux.Kem.Kyber.Sampling.sample_from_binomial_distribution (Rust_primitives.unsize prf_output
+
+                <:
+                slice u8)
           in
           let error_as_ntt:array Libcrux.Kem.Kyber.Arithmetic.t_KyberPolynomialRingElement v_K =
             Rust_primitives.Hax.update_at error_as_ntt
@@ -397,56 +418,58 @@ let generate_keypair
           in
           domain_separator, error_as_ntt, prf_input)
   in
-  let tt_as_ntt:array Libcrux.Kem.Kyber.Arithmetic.t_KyberPolynomialRingElement v_K =
+  let t__as_ntt:array Libcrux.Kem.Kyber.Arithmetic.t_KyberPolynomialRingElement v_K =
     Libcrux.Kem.Kyber.Ntt.multiply_matrix_by_column v_A_transpose secret_as_ntt
   in
-  let tt_as_ntt:array Libcrux.Kem.Kyber.Arithmetic.t_KyberPolynomialRingElement v_K =
-    Core.Iter.Traits.Iterator.Iterator.fold (Core.Iter.Traits.Collect.f_into_iter ({
-              Core.Ops.Range.f_start = sz 0;
-              Core.Ops.Range.f_end = v_K
+  let t__as_ntt:array Libcrux.Kem.Kyber.Arithmetic.t_KyberPolynomialRingElement v_K =
+    Core.Iter.Traits.Iterator.Iterator.fold (Core.Iter.Traits.Collect.IntoIterator.into_iter ({
+              Core.Ops.Range.Range.f_start = 0sz;
+              Core.Ops.Range.Range.f_end = v_K
             })
         <:
-        _.f_IntoIter)
-      tt_as_ntt
-      (fun tt_as_ntt i ->
-          Rust_primitives.Hax.update_at tt_as_ntt
+        _)
+      t__as_ntt
+      (fun t__as_ntt i ->
+          Rust_primitives.Hax.update_at t__as_ntt
             i
-            ((tt_as_ntt.[ i ] <: Libcrux.Kem.Kyber.Arithmetic.t_KyberPolynomialRingElement) +!
+            ((t__as_ntt.[ i ] <: Libcrux.Kem.Kyber.Arithmetic.t_KyberPolynomialRingElement) +.
               (error_as_ntt.[ i ] <: Libcrux.Kem.Kyber.Arithmetic.t_KyberPolynomialRingElement)
               <:
-              (Libcrux.Kem.Kyber.Arithmetic.t_impl_3).f_Output)
+              _)
           <:
           array Libcrux.Kem.Kyber.Arithmetic.t_KyberPolynomialRingElement v_K)
   in
   let public_key_serialized:Libcrux.Kem.Kyber.Conversions.t_UpdatableArray v_PUBLIC_KEY_SIZE =
-    Libcrux.Kem.Kyber.Conversions.impl__new (Rust_primitives.Hax.repeat 0uy v_PUBLIC_KEY_SIZE
+    Libcrux.Kem.Kyber.Conversions.new_under_impl (Rust_primitives.Hax.repeat 0uy v_PUBLIC_KEY_SIZE
         <:
         array u8 v_PUBLIC_KEY_SIZE)
   in
   let public_key_serialized:Libcrux.Kem.Kyber.Conversions.t_UpdatableArray v_PUBLIC_KEY_SIZE =
-    Libcrux.Kem.Kyber.Conversions.f_push public_key_serialized
-      (Rust_primitives.unsize (encode_12_ tt_as_ntt <: array u8 v_BYTES_PER_RING_ELEMENT)
+    Libcrux.Kem.Kyber.Conversions.UpdatingArray.push public_key_serialized
+      (Rust_primitives.unsize (encode_12_ t__as_ntt <: array u8 v_BYTES_PER_RING_ELEMENT)
         <:
         slice u8)
   in
   let public_key_serialized:array u8 v_PUBLIC_KEY_SIZE =
-    Libcrux.Kem.Kyber.Conversions.impl__array (Libcrux.Kem.Kyber.Conversions.f_push public_key_serialized
+    Libcrux.Kem.Kyber.Conversions.array_under_impl (Libcrux.Kem.Kyber.Conversions.UpdatingArray.push
+          public_key_serialized
           seed_for_A
         <:
         Libcrux.Kem.Kyber.Conversions.t_UpdatableArray v_PUBLIC_KEY_SIZE)
   in
   let secret_key_serialized:array u8 v_PRIVATE_KEY_SIZE = encode_12_ secret_as_ntt in
-  FStar.Pervasives.Native.Mktuple2 (Core.Convert.f_into secret_key_serialized)
-    (Core.Convert.f_into public_key_serialized),
+  FStar.Pervasives.Native.Mktuple2 (Core.Convert.Into.into secret_key_serialized)
+    (Core.Convert.Into.into public_key_serialized),
   sampling_A_error
 
 let serialize_secret_key
-      (#v_SERIALIZED_KEY_LEN: usize)
+      (#serialized_key_len: usize)
       (private_key public_key implicit_rejection_value: slice u8)
     : array u8 v_SERIALIZED_KEY_LEN =
-  Libcrux.Kem.Kyber.Conversions.impl__array (Libcrux.Kem.Kyber.Conversions.f_push (Libcrux.Kem.Kyber.Conversions.f_push
-            (Libcrux.Kem.Kyber.Conversions.f_push (Libcrux.Kem.Kyber.Conversions.f_push (Libcrux.Kem.Kyber.Conversions.impl__new
-                        (Rust_primitives.Hax.repeat 0uy v_SERIALIZED_KEY_LEN
+  Libcrux.Kem.Kyber.Conversions.array_under_impl (Libcrux.Kem.Kyber.Conversions.UpdatingArray.push (Libcrux.Kem.Kyber.Conversions.UpdatingArray.push
+            (Libcrux.Kem.Kyber.Conversions.UpdatingArray.push (Libcrux.Kem.Kyber.Conversions.UpdatingArray.push
+                    (Libcrux.Kem.Kyber.Conversions.new_under_impl (Rust_primitives.Hax.repeat 0uy
+                            v_SERIALIZED_KEY_LEN
                           <:
                           array u8 v_SERIALIZED_KEY_LEN)
                       <:
@@ -459,7 +482,7 @@ let serialize_secret_key
               Libcrux.Kem.Kyber.Conversions.t_UpdatableArray v_SERIALIZED_KEY_LEN)
             (Rust_primitives.unsize (Libcrux.Kem.Kyber.Hash_functions.v_H public_key
                   <:
-                  array u8 (sz 32))
+                  array u8 32sz)
               <:
               slice u8)
           <:
@@ -469,32 +492,34 @@ let serialize_secret_key
       Libcrux.Kem.Kyber.Conversions.t_UpdatableArray v_SERIALIZED_KEY_LEN)
 
 let compress_then_encode_u
-      (#v_K #v_OUT_LEN #v_COMPRESSION_FACTOR #v_BLOCK_LEN: usize)
+      (#k #out_len #compression_factor #block_len: usize)
       (input: array Libcrux.Kem.Kyber.Arithmetic.t_KyberPolynomialRingElement v_K)
     : array u8 v_OUT_LEN =
   let out:array u8 v_OUT_LEN = Rust_primitives.Hax.repeat 0uy v_OUT_LEN in
   let out:array u8 v_OUT_LEN =
-    Core.Iter.Traits.Iterator.Iterator.fold (Core.Iter.Traits.Collect.f_into_iter (Core.Iter.Traits.Iterator.f_enumerate
-              (Core.Iter.Traits.Collect.f_into_iter input <: _.f_IntoIter)
+    Core.Iter.Traits.Iterator.Iterator.fold (Core.Iter.Traits.Collect.IntoIterator.into_iter (Core.Iter.Traits.Iterator.Iterator.enumerate
+              (Core.Iter.Traits.Collect.IntoIterator.into_iter input <: _)
             <:
             Core.Iter.Adapters.Enumerate.t_Enumerate
             (Core.Array.Iter.t_IntoIter Libcrux.Kem.Kyber.Arithmetic.t_KyberPolynomialRingElement
                 v_K))
         <:
-        _.f_IntoIter)
+        _)
       out
       (fun out (i, re) ->
           Rust_primitives.Hax.update_at out
             ({
-                Core.Ops.Range.f_start = i *! (v_OUT_LEN /! v_K <: usize) <: usize;
-                Core.Ops.Range.f_end = (i +! sz 1 <: usize) *! (v_OUT_LEN /! v_K <: usize) <: usize
+                Core.Ops.Range.Range.f_start = i *. (v_OUT_LEN /. v_K <: usize) <: usize;
+                Core.Ops.Range.Range.f_end
+                =
+                (i +. 1sz <: usize) *. (v_OUT_LEN /. v_K <: usize) <: usize
               })
-            (Core.Slice.impl__copy_from_slice (Core.Ops.Index.IndexMut.index_mut out
+            (Core.Slice.copy_from_slice_under_impl (Core.Ops.Index.IndexMut.index_mut out
                     ({
-                        Core.Ops.Range.f_start = i *! (v_OUT_LEN /! v_K <: usize) <: usize;
-                        Core.Ops.Range.f_end
+                        Core.Ops.Range.Range.f_start = i *. (v_OUT_LEN /. v_K <: usize) <: usize;
+                        Core.Ops.Range.Range.f_end
                         =
-                        (i +! sz 1 <: usize) *! (v_OUT_LEN /! v_K <: usize) <: usize
+                        (i +. 1sz <: usize) *. (v_OUT_LEN /. v_K <: usize) <: usize
                       })
                   <:
                   slice u8)
@@ -514,20 +539,20 @@ let compress_then_encode_u
   out
 
 let encrypt
-      (#v_K #v_CIPHERTEXT_SIZE #v_T_AS_NTT_ENCODED_SIZE #v_C1_LEN #v_C2_LEN #v_VECTOR_U_COMPRESSION_FACTOR #v_VECTOR_V_COMPRESSION_FACTOR #v_BLOCK_LEN:
+      (#k #ciphertext_size #t__as_ntt_encoded_size #c1_len #c2_len #vector_u_compression_factor #vector_v_compression_factor #block_len #eta1 #eta1_randomness_size #eta2 #eta2_randomness_size:
           usize)
       (public_key: slice u8)
-      (message: array u8 (sz 32))
+      (message: array u8 32sz)
       (randomness: slice u8)
     : (Libcrux.Kem.Kyber.t_KyberCiphertext v_CIPHERTEXT_SIZE &
       Core.Option.t_Option Libcrux.Kem.Kyber.t_BadRejectionSamplingRandomnessError) =
-  let tt_as_ntt:array Libcrux.Kem.Kyber.Arithmetic.t_KyberPolynomialRingElement v_K =
-    Rust_primitives.Hax.repeat Libcrux.Kem.Kyber.Arithmetic.impl__ZERO v_K
+  let t__as_ntt:array Libcrux.Kem.Kyber.Arithmetic.t_KyberPolynomialRingElement v_K =
+    Rust_primitives.Hax.repeat Libcrux.Kem.Kyber.Arithmetic.v_ZERO_under_impl v_K
   in
-  let tt_as_ntt:array Libcrux.Kem.Kyber.Arithmetic.t_KyberPolynomialRingElement v_K =
-    Core.Iter.Traits.Iterator.Iterator.fold (Core.Iter.Traits.Collect.f_into_iter (Core.Iter.Traits.Iterator.f_enumerate
-              (Core.Slice.impl__chunks_exact (public_key.[ {
-                        Core.Ops.Range.f_end = v_T_AS_NTT_ENCODED_SIZE
+  let t__as_ntt:array Libcrux.Kem.Kyber.Arithmetic.t_KyberPolynomialRingElement v_K =
+    Core.Iter.Traits.Iterator.Iterator.fold (Core.Iter.Traits.Collect.IntoIterator.into_iter (Core.Iter.Traits.Iterator.Iterator.enumerate
+              (Core.Slice.chunks_exact_under_impl (public_key.[ {
+                        Core.Ops.Range.RangeTo.f_end = v_T_AS_NTT_ENCODED_SIZE
                       } ]
                     <:
                     slice u8)
@@ -537,24 +562,26 @@ let encrypt
             <:
             Core.Iter.Adapters.Enumerate.t_Enumerate (Core.Slice.Iter.t_ChunksExact u8))
         <:
-        _.f_IntoIter)
-      tt_as_ntt
-      (fun tt_as_ntt (i, tt_as_ntt_bytes) ->
-          Rust_primitives.Hax.update_at tt_as_ntt
+        _)
+      t__as_ntt
+      (fun t__as_ntt (i, t__as_ntt_bytes) ->
+          Rust_primitives.Hax.update_at t__as_ntt
             i
-            (Libcrux.Kem.Kyber.Serialize.deserialize_little_endian tt_as_ntt_bytes
+            (Libcrux.Kem.Kyber.Serialize.deserialize_little_endian t__as_ntt_bytes
               <:
               Libcrux.Kem.Kyber.Arithmetic.t_KyberPolynomialRingElement)
           <:
           array Libcrux.Kem.Kyber.Arithmetic.t_KyberPolynomialRingElement v_K)
   in
-  let seed:slice u8 = public_key.[ { Core.Ops.Range.f_start = v_T_AS_NTT_ENCODED_SIZE } ] in
+  let seed:slice u8 =
+    public_key.[ { Core.Ops.Range.RangeFrom.f_start = v_T_AS_NTT_ENCODED_SIZE } ]
+  in
   let v_A_transpose, sampling_A_error:(array
       (array Libcrux.Kem.Kyber.Arithmetic.t_KyberPolynomialRingElement v_K) v_K &
     Core.Option.t_Option Libcrux.Kem.Kyber.t_BadRejectionSamplingRandomnessError) =
-    sample_matrix_A (Libcrux.Kem.Kyber.Conversions.into_padded_array seed <: array u8 (sz 34)) false
+    sample_matrix_A (Libcrux.Kem.Kyber.Conversions.into_padded_array seed <: array u8 34sz) false
   in
-  let (prf_input: array u8 (sz 33)):array u8 (sz 33) =
+  let (prf_input: array u8 33sz):array u8 33sz =
     Libcrux.Kem.Kyber.Conversions.into_padded_array randomness
   in
   let r_as_ntt, domain_separator:(array Libcrux.Kem.Kyber.Arithmetic.t_KyberPolynomialRingElement
@@ -563,54 +590,57 @@ let encrypt
     cbd prf_input
   in
   let error_1_:array Libcrux.Kem.Kyber.Arithmetic.t_KyberPolynomialRingElement v_K =
-    Rust_primitives.Hax.repeat Libcrux.Kem.Kyber.Arithmetic.impl__ZERO v_K
+    Rust_primitives.Hax.repeat Libcrux.Kem.Kyber.Arithmetic.v_ZERO_under_impl v_K
   in
   let domain_separator, error_1_, prf_input:(Prims.unit &
     array Libcrux.Kem.Kyber.Arithmetic.t_KyberPolynomialRingElement v_K &
-    array u8 (sz 33)) =
-    Core.Iter.Traits.Iterator.Iterator.fold (Core.Iter.Traits.Collect.f_into_iter ({
-              Core.Ops.Range.f_start = sz 0;
-              Core.Ops.Range.f_end = v_K
+    array u8 33sz) =
+    Core.Iter.Traits.Iterator.Iterator.fold (Core.Iter.Traits.Collect.IntoIterator.into_iter ({
+              Core.Ops.Range.Range.f_start = 0sz;
+              Core.Ops.Range.Range.f_end = v_K
             })
         <:
-        _.f_IntoIter)
+        _)
       (domain_separator, error_1_, prf_input)
       (fun (domain_separator, error_1_, prf_input) i ->
-          let prf_input:array u8 (sz 33) =
-            Rust_primitives.Hax.update_at prf_input (sz 32) domain_separator
+          let prf_input:array u8 33sz =
+            Rust_primitives.Hax.update_at prf_input 32sz domain_separator
           in
-          let domain_separator:Prims.unit = domain_separator +! 1uy in
-          let (prf_output: array u8 (sz 128)):array u8 (sz 128) =
+          let domain_separator:Prims.unit = domain_separator +. 1uy in
+          let (prf_output: array u8 v_ETA2_RANDOMNESS_SIZE):array u8 v_ETA2_RANDOMNESS_SIZE =
             Libcrux.Kem.Kyber.Hash_functions.v_PRF (Rust_primitives.unsize prf_input <: slice u8)
           in
           let error_1_:array Libcrux.Kem.Kyber.Arithmetic.t_KyberPolynomialRingElement v_K =
             Rust_primitives.Hax.update_at error_1_
               i
-              (Libcrux.Kem.Kyber.Sampling.sample_from_binomial_distribution_2_ prf_output
+              (Libcrux.Kem.Kyber.Sampling.sample_from_binomial_distribution (Rust_primitives.unsize prf_output
+
+                    <:
+                    slice u8)
                 <:
                 Libcrux.Kem.Kyber.Arithmetic.t_KyberPolynomialRingElement)
           in
           domain_separator, error_1_, prf_input)
   in
-  let prf_input:array u8 (sz 33) =
-    Rust_primitives.Hax.update_at prf_input (sz 32) domain_separator
-  in
-  let (prf_output: array u8 (sz 128)):array u8 (sz 128) =
+  let prf_input:array u8 33sz = Rust_primitives.Hax.update_at prf_input 32sz domain_separator in
+  let (prf_output: array u8 v_ETA2_RANDOMNESS_SIZE):array u8 v_ETA2_RANDOMNESS_SIZE =
     Libcrux.Kem.Kyber.Hash_functions.v_PRF (Rust_primitives.unsize prf_input <: slice u8)
   in
   let error_2_:Libcrux.Kem.Kyber.Arithmetic.t_KyberPolynomialRingElement =
-    Libcrux.Kem.Kyber.Sampling.sample_from_binomial_distribution_2_ prf_output
+    Libcrux.Kem.Kyber.Sampling.sample_from_binomial_distribution (Rust_primitives.unsize prf_output
+        <:
+        slice u8)
   in
   let u:array Libcrux.Kem.Kyber.Arithmetic.t_KyberPolynomialRingElement v_K =
     Libcrux.Kem.Kyber.Ntt.multiply_matrix_by_column_montgomery v_A_transpose r_as_ntt
   in
   let u:array Libcrux.Kem.Kyber.Arithmetic.t_KyberPolynomialRingElement v_K =
-    Core.Iter.Traits.Iterator.Iterator.fold (Core.Iter.Traits.Collect.f_into_iter ({
-              Core.Ops.Range.f_start = sz 0;
-              Core.Ops.Range.f_end = v_K
+    Core.Iter.Traits.Iterator.Iterator.fold (Core.Iter.Traits.Collect.IntoIterator.into_iter ({
+              Core.Ops.Range.Range.f_start = 0sz;
+              Core.Ops.Range.Range.f_end = v_K
             })
         <:
-        _.f_IntoIter)
+        _)
       u
       (fun u i ->
           Rust_primitives.Hax.update_at u
@@ -619,10 +649,10 @@ let encrypt
                     <:
                     Libcrux.Kem.Kyber.Arithmetic.t_KyberPolynomialRingElement)
                 <:
-                Libcrux.Kem.Kyber.Arithmetic.t_KyberPolynomialRingElement) +!
+                Libcrux.Kem.Kyber.Arithmetic.t_KyberPolynomialRingElement) +.
               (error_1_.[ i ] <: Libcrux.Kem.Kyber.Arithmetic.t_KyberPolynomialRingElement)
               <:
-              (Libcrux.Kem.Kyber.Arithmetic.t_impl_3).f_Output)
+              _)
           <:
           array Libcrux.Kem.Kyber.Arithmetic.t_KyberPolynomialRingElement v_K)
   in
@@ -633,16 +663,16 @@ let encrypt
   in
   let v =
     ((Libcrux.Kem.Kyber.Ntt.invert_ntt_montgomery (Libcrux.Kem.Kyber.Ntt.multiply_row_by_column_montgomery
-              tt_as_ntt
+              t__as_ntt
               r_as_ntt
             <:
             Libcrux.Kem.Kyber.Arithmetic.t_KyberPolynomialRingElement)
         <:
-        Libcrux.Kem.Kyber.Arithmetic.t_KyberPolynomialRingElement) +!
+        Libcrux.Kem.Kyber.Arithmetic.t_KyberPolynomialRingElement) +.
       error_2_
       <:
-      (Libcrux.Kem.Kyber.Arithmetic.t_impl_3).f_Output) +!
-    (Libcrux.Kem.Kyber.Compress.decompress message_as_ring_element (sz 1)
+      _) +.
+    (Libcrux.Kem.Kyber.Compress.decompress message_as_ring_element 1sz
       <:
       Libcrux.Kem.Kyber.Arithmetic.t_KyberPolynomialRingElement)
   in
@@ -657,41 +687,41 @@ let encrypt
   in
   let ciphertext:array u8 v_CIPHERTEXT_SIZE =
     Rust_primitives.Hax.update_at ciphertext
-      ({ Core.Ops.Range.f_start = v_C1_LEN })
-      (Core.Slice.impl__copy_from_slice (Core.Ops.Index.IndexMut.index_mut ciphertext
-              ({ Core.Ops.Range.f_start = v_C1_LEN })
+      ({ Core.Ops.Range.RangeFrom.f_start = v_C1_LEN })
+      (Core.Slice.copy_from_slice_under_impl (Core.Ops.Index.IndexMut.index_mut ciphertext
+              ({ Core.Ops.Range.RangeFrom.f_start = v_C1_LEN })
             <:
             slice u8)
-          (Core.Array.impl_23__as_slice c2 <: slice u8)
+          (Core.Array.as_slice_under_impl_23 c2 <: slice u8)
         <:
         slice u8)
   in
-  Core.Convert.f_into ciphertext, sampling_A_error
+  Core.Convert.Into.into ciphertext, sampling_A_error
 
 let decrypt
-      (#v_K #v_CIPHERTEXT_SIZE #v_VECTOR_U_ENCODED_SIZE #v_VECTOR_U_COMPRESSION_FACTOR #v_VECTOR_V_COMPRESSION_FACTOR:
+      (#k #ciphertext_size #vector_u_encoded_size #vector_u_compression_factor #vector_v_compression_factor:
           usize)
       (secret_key: slice u8)
       (ciphertext: Libcrux.Kem.Kyber.t_KyberCiphertext v_CIPHERTEXT_SIZE)
-    : array u8 (sz 32) =
+    : array u8 32sz =
   let u_as_ntt:array Libcrux.Kem.Kyber.Arithmetic.t_KyberPolynomialRingElement v_K =
-    Rust_primitives.Hax.repeat Libcrux.Kem.Kyber.Arithmetic.impl__ZERO v_K
+    Rust_primitives.Hax.repeat Libcrux.Kem.Kyber.Arithmetic.v_ZERO_under_impl v_K
   in
   let secret_as_ntt:array Libcrux.Kem.Kyber.Arithmetic.t_KyberPolynomialRingElement v_K =
-    Rust_primitives.Hax.repeat Libcrux.Kem.Kyber.Arithmetic.impl__ZERO v_K
+    Rust_primitives.Hax.repeat Libcrux.Kem.Kyber.Arithmetic.v_ZERO_under_impl v_K
   in
   let u_as_ntt:array Libcrux.Kem.Kyber.Arithmetic.t_KyberPolynomialRingElement v_K =
-    Core.Iter.Traits.Iterator.Iterator.fold (Core.Iter.Traits.Collect.f_into_iter (Core.Iter.Traits.Iterator.f_enumerate
-              (Core.Slice.impl__chunks_exact (ciphertext.[ {
-                        Core.Ops.Range.f_end = v_VECTOR_U_ENCODED_SIZE
+    Core.Iter.Traits.Iterator.Iterator.fold (Core.Iter.Traits.Collect.IntoIterator.into_iter (Core.Iter.Traits.Iterator.Iterator.enumerate
+              (Core.Slice.chunks_exact_under_impl (ciphertext.[ {
+                        Core.Ops.Range.RangeTo.f_end = v_VECTOR_U_ENCODED_SIZE
                       } ]
                     <:
                     slice u8)
-                  ((Libcrux.Kem.Kyber.Constants.v_COEFFICIENTS_IN_RING_ELEMENT *!
+                  ((Libcrux.Kem.Kyber.Constants.v_COEFFICIENTS_IN_RING_ELEMENT *.
                       v_VECTOR_U_COMPRESSION_FACTOR
                       <:
-                      usize) /!
-                    sz 8
+                      usize) /.
+                    8sz
                     <:
                     usize)
                 <:
@@ -699,19 +729,20 @@ let decrypt
             <:
             Core.Iter.Adapters.Enumerate.t_Enumerate (Core.Slice.Iter.t_ChunksExact u8))
         <:
-        _.f_IntoIter)
+        _)
       u_as_ntt
       (fun u_as_ntt (i, u_bytes) ->
           let u:Libcrux.Kem.Kyber.Arithmetic.t_KyberPolynomialRingElement =
-            Libcrux.Kem.Kyber.Serialize.deserialize_little_endian u_bytes
+            Libcrux.Kem.Kyber.Compress.decompress (Libcrux.Kem.Kyber.Serialize.deserialize_little_endian
+                  u_bytes
+                <:
+                Libcrux.Kem.Kyber.Arithmetic.t_KyberPolynomialRingElement)
+              v_VECTOR_U_COMPRESSION_FACTOR
           in
           let u_as_ntt:array Libcrux.Kem.Kyber.Arithmetic.t_KyberPolynomialRingElement v_K =
             Rust_primitives.Hax.update_at u_as_ntt
               i
-              (Libcrux.Kem.Kyber.Ntt.ntt_representation (Libcrux.Kem.Kyber.Compress.decompress u
-                      (sz 10)
-                    <:
-                    Libcrux.Kem.Kyber.Arithmetic.t_KyberPolynomialRingElement)
+              (Libcrux.Kem.Kyber.Ntt.ntt_representation u
                 <:
                 Libcrux.Kem.Kyber.Arithmetic.t_KyberPolynomialRingElement)
           in
@@ -719,7 +750,7 @@ let decrypt
   in
   let v:Libcrux.Kem.Kyber.Arithmetic.t_KyberPolynomialRingElement =
     Libcrux.Kem.Kyber.Compress.decompress (Libcrux.Kem.Kyber.Serialize.deserialize_little_endian (ciphertext.[
-              { Core.Ops.Range.f_start = v_VECTOR_U_ENCODED_SIZE } ]
+              { Core.Ops.Range.RangeFrom.f_start = v_VECTOR_U_ENCODED_SIZE } ]
             <:
             slice u8)
         <:
@@ -727,15 +758,15 @@ let decrypt
       v_VECTOR_V_COMPRESSION_FACTOR
   in
   let secret_as_ntt:array Libcrux.Kem.Kyber.Arithmetic.t_KyberPolynomialRingElement v_K =
-    Core.Iter.Traits.Iterator.Iterator.fold (Core.Iter.Traits.Collect.f_into_iter (Core.Iter.Traits.Iterator.f_enumerate
-              (Core.Slice.impl__chunks_exact secret_key
+    Core.Iter.Traits.Iterator.Iterator.fold (Core.Iter.Traits.Collect.IntoIterator.into_iter (Core.Iter.Traits.Iterator.Iterator.enumerate
+              (Core.Slice.chunks_exact_under_impl secret_key
                   Libcrux.Kem.Kyber.Constants.v_BYTES_PER_RING_ELEMENT
                 <:
                 Core.Slice.Iter.t_ChunksExact u8)
             <:
             Core.Iter.Adapters.Enumerate.t_Enumerate (Core.Slice.Iter.t_ChunksExact u8))
         <:
-        _.f_IntoIter)
+        _)
       secret_as_ntt
       (fun secret_as_ntt (i, secret_bytes) ->
           Rust_primitives.Hax.update_at secret_as_ntt
@@ -747,7 +778,7 @@ let decrypt
           array Libcrux.Kem.Kyber.Arithmetic.t_KyberPolynomialRingElement v_K)
   in
   let message =
-    v -!
+    v -.
     (Libcrux.Kem.Kyber.Ntt.invert_ntt_montgomery (Libcrux.Kem.Kyber.Ntt.multiply_row_by_column_montgomery
             secret_as_ntt
             u_as_ntt
