proofs/fstar/extraction/Libcrux.Kem.Kyber.fst
@@ -2,396 +2,444 @@ module Libcrux.Kem.Kyber
 #set-options "--fuel 0 --ifuel 1 --z3rlimit 15"
 open Core
 
-type t_KyberCiphertext (#v_SIZE: usize) = { f_value:array u8 v_SIZE }
+type t_KyberCiphertext = { f_value:array u8 v_SIZE }
 
-let impl (#v_SIZE: usize) : Core.Convert.t_AsRef (t_KyberCiphertext v_SIZE) (slice u8) =
+let impl (#size: usize) : Core.Convert.t_AsRef (t_KyberCiphertext v_SIZE) (slice u8) =
   {
-    f_impl__as_ref
+    as_ref
     =
-    fun (#v_SIZE: usize) (self: t_KyberCiphertext v_SIZE) -> Rust_primitives.unsize self.f_value
+    fun (#size: usize) (self: t_KyberCiphertext v_SIZE) ->
+      Rust_primitives.unsize self.Libcrux.Kem.Kyber.KyberCiphertext.f_value
   }
 
-let impl_1 (#v_SIZE: usize) : Core.Convert.t_From (t_KyberCiphertext v_SIZE) (array u8 v_SIZE) =
-  { f_impl_1__from = fun (#v_SIZE: usize) (value: array u8 v_SIZE) -> { f_value = value } }
-
-let impl_2 (#v_SIZE: usize) : Core.Convert.t_From (array u8 v_SIZE) (t_KyberCiphertext v_SIZE) =
-  { f_impl_2__from = fun (#v_SIZE: usize) (value: t_KyberCiphertext v_SIZE) -> value.f_value }
-
-let impl_3 (#v_SIZE: usize) : Core.Convert.t_TryFrom (t_KyberCiphertext v_SIZE) (slice u8) =
+let impl (#size: usize) : Core.Convert.t_From (t_KyberCiphertext v_SIZE) (array u8 v_SIZE) =
   {
-    f_impl_3__Error = Core.Array.t_TryFromSliceError;
-    f_impl_3__try_from
+    from
     =
-    fun (#v_SIZE: usize) (value: slice u8) ->
+    fun (#size: usize) (value: array u8 v_SIZE) ->
+      { Libcrux.Kem.Kyber.KyberCiphertext.f_value = value }
+  }
+
+let impl (#size: usize) : Core.Convert.t_From (array u8 v_SIZE) (t_KyberCiphertext v_SIZE) =
+  {
+    from
+    =
+    fun (#size: usize) (value: t_KyberCiphertext v_SIZE) ->
+      value.Libcrux.Kem.Kyber.KyberCiphertext.f_value
+  }
+
+let impl (#size: usize) : Core.Convert.t_TryFrom (t_KyberCiphertext v_SIZE) (slice u8) =
+  {
+    error = Core.Array.t_TryFromSliceError;
+    try_from
+    =
+    fun (#size: usize) (value: slice u8) ->
       Rust_primitives.Hax.Control_flow_monad.Mexception.run (let* hoist6:array u8 v_SIZE =
             match
-              Core.Ops.Try_trait.f_branch (Core.Convert.f_try_into value
+              Core.Ops.Try_trait.Try.branch (Core.Convert.TryInto.try_into value
                   <:
-                  Core.Result.t_Result (array u8 v_SIZE) _.f_Error)
+                  Core.Result.t_Result (array u8 v_SIZE) _)
             with
-            | Core.Ops.Control_flow.ControlFlow_Break
-              { Core.Ops.Control_flow.ControlFlow._0 = residual } ->
+            | Core.Ops.Control_flow.ControlFlow_Break residual ->
               let* hoist5:Rust_primitives.Hax.t_Never =
-                Core.Ops.Control_flow.ControlFlow.v_Break (Core.Ops.Try_trait.f_from_residual residual
-
+                Core.Ops.Control_flow.ControlFlow.v_Break (Core.Ops.Try_trait.FromResidual.from_residual
+                      residual
                     <:
                     Core.Result.t_Result (t_KyberCiphertext v_SIZE) Core.Array.t_TryFromSliceError)
               in
               Core.Ops.Control_flow.ControlFlow_Continue (Rust_primitives.Hax.never_to_any hoist5)
-            | Core.Ops.Control_flow.ControlFlow_Continue
-              { Core.Ops.Control_flow.ControlFlow._0 = v_val } ->
+            | Core.Ops.Control_flow.ControlFlow_Continue v_val ->
               Core.Ops.Control_flow.ControlFlow_Continue v_val
           in
           Core.Ops.Control_flow.ControlFlow_Continue
-          (let hoist7:t_KyberCiphertext v_SIZE = { f_value = hoist6 } in
+          (let hoist7:t_KyberCiphertext v_SIZE =
+              { Libcrux.Kem.Kyber.KyberCiphertext.f_value = hoist6 }
+            in
             Core.Result.Result_Ok hoist7))
   }
 
-let impl_4 (#v_SIZE: usize) : Core.Ops.Index.t_Index (t_KyberCiphertext v_SIZE) usize =
+let impl (#size: usize) : Core.Ops.Index.t_Index (t_KyberCiphertext v_SIZE) usize =
   {
-    f_impl_4__Output = u8;
-    f_impl_4__index
+    output = u8;
+    index
     =
-    fun (#v_SIZE: usize) (self: t_KyberCiphertext v_SIZE) (index: usize) -> self.f_value.[ index ]
+    fun (#size: usize) (self: t_KyberCiphertext v_SIZE) (index: usize) ->
+      self.Libcrux.Kem.Kyber.KyberCiphertext.f_value.[ index ]
   }
 
-let impl_5 (#v_SIZE: usize)
+let impl (#size: usize)
     : Core.Ops.Index.t_Index (t_KyberCiphertext v_SIZE) (Core.Ops.Range.t_Range usize) =
   {
-    f_impl_5__Output = slice u8;
-    f_impl_5__index
+    output = slice u8;
+    index
     =
-    fun (#v_SIZE: usize) (self: t_KyberCiphertext v_SIZE) (range: Core.Ops.Range.t_Range usize) ->
-      self.f_value.[ range ]
+    fun (#size: usize) (self: t_KyberCiphertext v_SIZE) (range: Core.Ops.Range.t_Range usize) ->
+      self.Libcrux.Kem.Kyber.KyberCiphertext.f_value.[ range ]
   }
 
-let impl_6 (#v_SIZE: usize)
+let impl (#size: usize)
     : Core.Ops.Index.t_Index (t_KyberCiphertext v_SIZE) (Core.Ops.Range.t_RangeTo usize) =
   {
-    f_impl_6__Output = slice u8;
-    f_impl_6__index
+    output = slice u8;
+    index
     =
-    fun (#v_SIZE: usize) (self: t_KyberCiphertext v_SIZE) (range: Core.Ops.Range.t_RangeTo usize) ->
-      self.f_value.[ range ]
+    fun (#size: usize) (self: t_KyberCiphertext v_SIZE) (range: Core.Ops.Range.t_RangeTo usize) ->
+      self.Libcrux.Kem.Kyber.KyberCiphertext.f_value.[ range ]
   }
 
-let impl_7 (#v_SIZE: usize)
+let impl (#size: usize)
     : Core.Ops.Index.t_Index (t_KyberCiphertext v_SIZE) (Core.Ops.Range.t_RangeFrom usize) =
   {
-    f_impl_7__Output = slice u8;
-    f_impl_7__index
+    output = slice u8;
+    index
     =
-    fun
-      (#v_SIZE: usize)
-      (self: t_KyberCiphertext v_SIZE)
-      (range: Core.Ops.Range.t_RangeFrom usize)
-      ->
-      self.f_value.[ range ]
+    fun (#size: usize) (self: t_KyberCiphertext v_SIZE) (range: Core.Ops.Range.t_RangeFrom usize) ->
+      self.Libcrux.Kem.Kyber.KyberCiphertext.f_value.[ range ]
   }
 
-let impl_8__as_slice (#v_SIZE: usize) (self: t_KyberCiphertext v_SIZE) : array u8 v_SIZE =
-  self.f_value
+let as_slice_under_impl_8 (#size: usize) (self: t_KyberCiphertext v_SIZE) : array u8 v_SIZE =
+  self.Libcrux.Kem.Kyber.KyberCiphertext.f_value
 
-let impl_8__split_at (#v_SIZE: usize) (self: t_KyberCiphertext v_SIZE) (mid: usize)
+let split_at_under_impl_8 (#size: usize) (self: t_KyberCiphertext v_SIZE) (mid: usize)
     : (slice u8 & slice u8) =
-  Core.Slice.impl__split_at (Rust_primitives.unsize self.f_value <: slice u8) mid
+  Core.Slice.split_at_under_impl (Rust_primitives.unsize self
+          .Libcrux.Kem.Kyber.KyberCiphertext.f_value
+      <:
+      slice u8)
+    mid
 
-let impl_8__len (#v_SIZE: usize) (self: t_KyberCiphertext v_SIZE) : usize = v_SIZE
+let len_under_impl_8 (#size: usize) (self: t_KyberCiphertext v_SIZE) : usize = v_SIZE
 
-type t_KyberSharedSecret (#v_SIZE: usize) = { f_value:array u8 v_SIZE }
+type t_KyberSharedSecret = { f_value:array u8 v_SIZE }
 
-let impl_9 (#v_SIZE: usize) : Core.Convert.t_AsRef (t_KyberSharedSecret v_SIZE) (slice u8) =
+let impl (#size: usize) : Core.Convert.t_AsRef (t_KyberSharedSecret v_SIZE) (slice u8) =
   {
-    f_impl_9__as_ref
+    as_ref
     =
-    fun (#v_SIZE: usize) (self: t_KyberSharedSecret v_SIZE) -> Rust_primitives.unsize self.f_value
+    fun (#size: usize) (self: t_KyberSharedSecret v_SIZE) ->
+      Rust_primitives.unsize self.Libcrux.Kem.Kyber.KyberSharedSecret.f_value
   }
 
-let impl_10 (#v_SIZE: usize) : Core.Convert.t_From (t_KyberSharedSecret v_SIZE) (array u8 v_SIZE) =
-  { f_impl_10__from = fun (#v_SIZE: usize) (value: array u8 v_SIZE) -> { f_value = value } }
-
-let impl_11 (#v_SIZE: usize) : Core.Convert.t_From (array u8 v_SIZE) (t_KyberSharedSecret v_SIZE) =
-  { f_impl_11__from = fun (#v_SIZE: usize) (value: t_KyberSharedSecret v_SIZE) -> value.f_value }
-
-let impl_12 (#v_SIZE: usize) : Core.Convert.t_TryFrom (t_KyberSharedSecret v_SIZE) (slice u8) =
+let impl (#size: usize) : Core.Convert.t_From (t_KyberSharedSecret v_SIZE) (array u8 v_SIZE) =
   {
-    f_impl_12__Error = Core.Array.t_TryFromSliceError;
-    f_impl_12__try_from
+    from
     =
-    fun (#v_SIZE: usize) (value: slice u8) ->
+    fun (#size: usize) (value: array u8 v_SIZE) ->
+      { Libcrux.Kem.Kyber.KyberSharedSecret.f_value = value }
+  }
+
+let impl (#size: usize) : Core.Convert.t_From (array u8 v_SIZE) (t_KyberSharedSecret v_SIZE) =
+  {
+    from
+    =
+    fun (#size: usize) (value: t_KyberSharedSecret v_SIZE) ->
+      value.Libcrux.Kem.Kyber.KyberSharedSecret.f_value
+  }
+
+let impl (#size: usize) : Core.Convert.t_TryFrom (t_KyberSharedSecret v_SIZE) (slice u8) =
+  {
+    error = Core.Array.t_TryFromSliceError;
+    try_from
+    =
+    fun (#size: usize) (value: slice u8) ->
       Rust_primitives.Hax.Control_flow_monad.Mexception.run (let* hoist9:array u8 v_SIZE =
             match
-              Core.Ops.Try_trait.f_branch (Core.Convert.f_try_into value
+              Core.Ops.Try_trait.Try.branch (Core.Convert.TryInto.try_into value
                   <:
-                  Core.Result.t_Result (array u8 v_SIZE) _.f_Error)
+                  Core.Result.t_Result (array u8 v_SIZE) _)
             with
-            | Core.Ops.Control_flow.ControlFlow_Break
-              { Core.Ops.Control_flow.ControlFlow._0 = residual } ->
+            | Core.Ops.Control_flow.ControlFlow_Break residual ->
               let* hoist8:Rust_primitives.Hax.t_Never =
-                Core.Ops.Control_flow.ControlFlow.v_Break (Core.Ops.Try_trait.f_from_residual residual
-
+                Core.Ops.Control_flow.ControlFlow.v_Break (Core.Ops.Try_trait.FromResidual.from_residual
+                      residual
                     <:
                     Core.Result.t_Result (t_KyberSharedSecret v_SIZE) Core.Array.t_TryFromSliceError
                   )
               in
               Core.Ops.Control_flow.ControlFlow_Continue (Rust_primitives.Hax.never_to_any hoist8)
-            | Core.Ops.Control_flow.ControlFlow_Continue
-              { Core.Ops.Control_flow.ControlFlow._0 = v_val } ->
+            | Core.Ops.Control_flow.ControlFlow_Continue v_val ->
               Core.Ops.Control_flow.ControlFlow_Continue v_val
           in
           Core.Ops.Control_flow.ControlFlow_Continue
-          (let hoist10:t_KyberSharedSecret v_SIZE = { f_value = hoist9 } in
+          (let hoist10:t_KyberSharedSecret v_SIZE =
+              { Libcrux.Kem.Kyber.KyberSharedSecret.f_value = hoist9 }
+            in
             Core.Result.Result_Ok hoist10))
   }
 
-let impl_13 (#v_SIZE: usize) : Core.Ops.Index.t_Index (t_KyberSharedSecret v_SIZE) usize =
+let impl (#size: usize) : Core.Ops.Index.t_Index (t_KyberSharedSecret v_SIZE) usize =
   {
-    f_impl_13__Output = u8;
-    f_impl_13__index
+    output = u8;
+    index
     =
-    fun (#v_SIZE: usize) (self: t_KyberSharedSecret v_SIZE) (index: usize) -> self.f_value.[ index ]
+    fun (#size: usize) (self: t_KyberSharedSecret v_SIZE) (index: usize) ->
+      self.Libcrux.Kem.Kyber.KyberSharedSecret.f_value.[ index ]
   }
 
-let impl_14 (#v_SIZE: usize)
+let impl (#size: usize)
     : Core.Ops.Index.t_Index (t_KyberSharedSecret v_SIZE) (Core.Ops.Range.t_Range usize) =
   {
-    f_impl_14__Output = slice u8;
-    f_impl_14__index
+    output = slice u8;
+    index
     =
-    fun (#v_SIZE: usize) (self: t_KyberSharedSecret v_SIZE) (range: Core.Ops.Range.t_Range usize) ->
-      self.f_value.[ range ]
+    fun (#size: usize) (self: t_KyberSharedSecret v_SIZE) (range: Core.Ops.Range.t_Range usize) ->
+      self.Libcrux.Kem.Kyber.KyberSharedSecret.f_value.[ range ]
   }
 
-let impl_15 (#v_SIZE: usize)
+let impl (#size: usize)
     : Core.Ops.Index.t_Index (t_KyberSharedSecret v_SIZE) (Core.Ops.Range.t_RangeTo usize) =
   {
-    f_impl_15__Output = slice u8;
-    f_impl_15__index
+    output = slice u8;
+    index
     =
-    fun
-      (#v_SIZE: usize)
-      (self: t_KyberSharedSecret v_SIZE)
-      (range: Core.Ops.Range.t_RangeTo usize)
-      ->
-      self.f_value.[ range ]
+    fun (#size: usize) (self: t_KyberSharedSecret v_SIZE) (range: Core.Ops.Range.t_RangeTo usize) ->
+      self.Libcrux.Kem.Kyber.KyberSharedSecret.f_value.[ range ]
   }
 
-let impl_16 (#v_SIZE: usize)
+let impl (#size: usize)
     : Core.Ops.Index.t_Index (t_KyberSharedSecret v_SIZE) (Core.Ops.Range.t_RangeFrom usize) =
   {
-    f_impl_16__Output = slice u8;
-    f_impl_16__index
+    output = slice u8;
+    index
     =
     fun
-      (#v_SIZE: usize)
+      (#size: usize)
       (self: t_KyberSharedSecret v_SIZE)
       (range: Core.Ops.Range.t_RangeFrom usize)
       ->
-      self.f_value.[ range ]
+      self.Libcrux.Kem.Kyber.KyberSharedSecret.f_value.[ range ]
   }
 
-let impl_17__as_slice (#v_SIZE: usize) (self: t_KyberSharedSecret v_SIZE) : array u8 v_SIZE =
-  self.f_value
+let as_slice_under_impl_17 (#size: usize) (self: t_KyberSharedSecret v_SIZE) : array u8 v_SIZE =
+  self.Libcrux.Kem.Kyber.KyberSharedSecret.f_value
 
-let impl_17__split_at (#v_SIZE: usize) (self: t_KyberSharedSecret v_SIZE) (mid: usize)
+let split_at_under_impl_17 (#size: usize) (self: t_KyberSharedSecret v_SIZE) (mid: usize)
     : (slice u8 & slice u8) =
-  Core.Slice.impl__split_at (Rust_primitives.unsize self.f_value <: slice u8) mid
+  Core.Slice.split_at_under_impl (Rust_primitives.unsize self
+          .Libcrux.Kem.Kyber.KyberSharedSecret.f_value
+      <:
+      slice u8)
+    mid
 
-let impl_17__len (#v_SIZE: usize) (self: t_KyberSharedSecret v_SIZE) : usize = v_SIZE
+let len_under_impl_17 (#size: usize) (self: t_KyberSharedSecret v_SIZE) : usize = v_SIZE
 
-type t_KyberPrivateKey (#v_SIZE: usize) = { f_value:array u8 v_SIZE }
+type t_KyberPrivateKey = { f_value:array u8 v_SIZE }
 
-let impl_18 (#v_SIZE: usize) : Core.Convert.t_AsRef (t_KyberPrivateKey v_SIZE) (slice u8) =
+let impl (#size: usize) : Core.Convert.t_AsRef (t_KyberPrivateKey v_SIZE) (slice u8) =
   {
-    f_impl_18__as_ref
+    as_ref
     =
-    fun (#v_SIZE: usize) (self: t_KyberPrivateKey v_SIZE) -> Rust_primitives.unsize self.f_value
+    fun (#size: usize) (self: t_KyberPrivateKey v_SIZE) ->
+      Rust_primitives.unsize self.Libcrux.Kem.Kyber.KyberPrivateKey.f_value
   }
 
-let impl_19 (#v_SIZE: usize) : Core.Convert.t_From (t_KyberPrivateKey v_SIZE) (array u8 v_SIZE) =
-  { f_impl_19__from = fun (#v_SIZE: usize) (value: array u8 v_SIZE) -> { f_value = value } }
-
-let impl_20 (#v_SIZE: usize) : Core.Convert.t_From (array u8 v_SIZE) (t_KyberPrivateKey v_SIZE) =
-  { f_impl_20__from = fun (#v_SIZE: usize) (value: t_KyberPrivateKey v_SIZE) -> value.f_value }
-
-let impl_21 (#v_SIZE: usize) : Core.Convert.t_TryFrom (t_KyberPrivateKey v_SIZE) (slice u8) =
+let impl (#size: usize) : Core.Convert.t_From (t_KyberPrivateKey v_SIZE) (array u8 v_SIZE) =
   {
-    f_impl_21__Error = Core.Array.t_TryFromSliceError;
-    f_impl_21__try_from
+    from
     =
-    fun (#v_SIZE: usize) (value: slice u8) ->
+    fun (#size: usize) (value: array u8 v_SIZE) ->
+      { Libcrux.Kem.Kyber.KyberPrivateKey.f_value = value }
+  }
+
+let impl (#size: usize) : Core.Convert.t_From (array u8 v_SIZE) (t_KyberPrivateKey v_SIZE) =
+  {
+    from
+    =
+    fun (#size: usize) (value: t_KyberPrivateKey v_SIZE) ->
+      value.Libcrux.Kem.Kyber.KyberPrivateKey.f_value
+  }
+
+let impl (#size: usize) : Core.Convert.t_TryFrom (t_KyberPrivateKey v_SIZE) (slice u8) =
+  {
+    error = Core.Array.t_TryFromSliceError;
+    try_from
+    =
+    fun (#size: usize) (value: slice u8) ->
       Rust_primitives.Hax.Control_flow_monad.Mexception.run (let* hoist12:array u8 v_SIZE =
             match
-              Core.Ops.Try_trait.f_branch (Core.Convert.f_try_into value
+              Core.Ops.Try_trait.Try.branch (Core.Convert.TryInto.try_into value
                   <:
-                  Core.Result.t_Result (array u8 v_SIZE) _.f_Error)
+                  Core.Result.t_Result (array u8 v_SIZE) _)
             with
-            | Core.Ops.Control_flow.ControlFlow_Break
-              { Core.Ops.Control_flow.ControlFlow._0 = residual } ->
+            | Core.Ops.Control_flow.ControlFlow_Break residual ->
               let* hoist11:Rust_primitives.Hax.t_Never =
-                Core.Ops.Control_flow.ControlFlow.v_Break (Core.Ops.Try_trait.f_from_residual residual
-
+                Core.Ops.Control_flow.ControlFlow.v_Break (Core.Ops.Try_trait.FromResidual.from_residual
+                      residual
                     <:
                     Core.Result.t_Result (t_KyberPrivateKey v_SIZE) Core.Array.t_TryFromSliceError)
               in
               Core.Ops.Control_flow.ControlFlow_Continue (Rust_primitives.Hax.never_to_any hoist11)
-            | Core.Ops.Control_flow.ControlFlow_Continue
-              { Core.Ops.Control_flow.ControlFlow._0 = v_val } ->
+            | Core.Ops.Control_flow.ControlFlow_Continue v_val ->
               Core.Ops.Control_flow.ControlFlow_Continue v_val
           in
           Core.Ops.Control_flow.ControlFlow_Continue
-          (let hoist13:t_KyberPrivateKey v_SIZE = { f_value = hoist12 } in
+          (let hoist13:t_KyberPrivateKey v_SIZE =
+              { Libcrux.Kem.Kyber.KyberPrivateKey.f_value = hoist12 }
+            in
             Core.Result.Result_Ok hoist13))
   }
 
-let impl_22 (#v_SIZE: usize) : Core.Ops.Index.t_Index (t_KyberPrivateKey v_SIZE) usize =
+let impl (#size: usize) : Core.Ops.Index.t_Index (t_KyberPrivateKey v_SIZE) usize =
   {
-    f_impl_22__Output = u8;
-    f_impl_22__index
+    output = u8;
+    index
     =
-    fun (#v_SIZE: usize) (self: t_KyberPrivateKey v_SIZE) (index: usize) -> self.f_value.[ index ]
+    fun (#size: usize) (self: t_KyberPrivateKey v_SIZE) (index: usize) ->
+      self.Libcrux.Kem.Kyber.KyberPrivateKey.f_value.[ index ]
   }
 
-let impl_23 (#v_SIZE: usize)
+let impl (#size: usize)
     : Core.Ops.Index.t_Index (t_KyberPrivateKey v_SIZE) (Core.Ops.Range.t_Range usize) =
   {
-    f_impl_23__Output = slice u8;
-    f_impl_23__index
+    output = slice u8;
+    index
     =
-    fun (#v_SIZE: usize) (self: t_KyberPrivateKey v_SIZE) (range: Core.Ops.Range.t_Range usize) ->
-      self.f_value.[ range ]
+    fun (#size: usize) (self: t_KyberPrivateKey v_SIZE) (range: Core.Ops.Range.t_Range usize) ->
+      self.Libcrux.Kem.Kyber.KyberPrivateKey.f_value.[ range ]
   }
 
-let impl_24 (#v_SIZE: usize)
+let impl (#size: usize)
     : Core.Ops.Index.t_Index (t_KyberPrivateKey v_SIZE) (Core.Ops.Range.t_RangeTo usize) =
   {
-    f_impl_24__Output = slice u8;
-    f_impl_24__index
+    output = slice u8;
+    index
     =
-    fun (#v_SIZE: usize) (self: t_KyberPrivateKey v_SIZE) (range: Core.Ops.Range.t_RangeTo usize) ->
-      self.f_value.[ range ]
+    fun (#size: usize) (self: t_KyberPrivateKey v_SIZE) (range: Core.Ops.Range.t_RangeTo usize) ->
+      self.Libcrux.Kem.Kyber.KyberPrivateKey.f_value.[ range ]
   }
 
-let impl_25 (#v_SIZE: usize)
+let impl (#size: usize)
     : Core.Ops.Index.t_Index (t_KyberPrivateKey v_SIZE) (Core.Ops.Range.t_RangeFrom usize) =
   {
-    f_impl_25__Output = slice u8;
-    f_impl_25__index
+    output = slice u8;
+    index
     =
-    fun
-      (#v_SIZE: usize)
-      (self: t_KyberPrivateKey v_SIZE)
-      (range: Core.Ops.Range.t_RangeFrom usize)
-      ->
-      self.f_value.[ range ]
+    fun (#size: usize) (self: t_KyberPrivateKey v_SIZE) (range: Core.Ops.Range.t_RangeFrom usize) ->
+      self.Libcrux.Kem.Kyber.KyberPrivateKey.f_value.[ range ]
   }
 
-let impl_26__as_slice (#v_SIZE: usize) (self: t_KyberPrivateKey v_SIZE) : array u8 v_SIZE =
-  self.f_value
+let as_slice_under_impl_26 (#size: usize) (self: t_KyberPrivateKey v_SIZE) : array u8 v_SIZE =
+  self.Libcrux.Kem.Kyber.KyberPrivateKey.f_value
 
-let impl_26__split_at (#v_SIZE: usize) (self: t_KyberPrivateKey v_SIZE) (mid: usize)
+let split_at_under_impl_26 (#size: usize) (self: t_KyberPrivateKey v_SIZE) (mid: usize)
     : (slice u8 & slice u8) =
-  Core.Slice.impl__split_at (Rust_primitives.unsize self.f_value <: slice u8) mid
+  Core.Slice.split_at_under_impl (Rust_primitives.unsize self
+          .Libcrux.Kem.Kyber.KyberPrivateKey.f_value
+      <:
+      slice u8)
+    mid
 
-let impl_26__len (#v_SIZE: usize) (self: t_KyberPrivateKey v_SIZE) : usize = v_SIZE
+let len_under_impl_26 (#size: usize) (self: t_KyberPrivateKey v_SIZE) : usize = v_SIZE
 
-type t_KyberPublicKey (#v_SIZE: usize) = { f_value:array u8 v_SIZE }
+type t_KyberPublicKey = { f_value:array u8 v_SIZE }
 
-let impl_27 (#v_SIZE: usize) : Core.Convert.t_AsRef (t_KyberPublicKey v_SIZE) (slice u8) =
+let impl (#size: usize) : Core.Convert.t_AsRef (t_KyberPublicKey v_SIZE) (slice u8) =
   {
-    f_impl_27__as_ref
+    as_ref
     =
-    fun (#v_SIZE: usize) (self: t_KyberPublicKey v_SIZE) -> Rust_primitives.unsize self.f_value
+    fun (#size: usize) (self: t_KyberPublicKey v_SIZE) ->
+      Rust_primitives.unsize self.Libcrux.Kem.Kyber.KyberPublicKey.f_value
   }
 
-let impl_28 (#v_SIZE: usize) : Core.Convert.t_From (t_KyberPublicKey v_SIZE) (array u8 v_SIZE) =
-  { f_impl_28__from = fun (#v_SIZE: usize) (value: array u8 v_SIZE) -> { f_value = value } }
-
-let impl_29 (#v_SIZE: usize) : Core.Convert.t_From (array u8 v_SIZE) (t_KyberPublicKey v_SIZE) =
-  { f_impl_29__from = fun (#v_SIZE: usize) (value: t_KyberPublicKey v_SIZE) -> value.f_value }
-
-let impl_30 (#v_SIZE: usize) : Core.Convert.t_TryFrom (t_KyberPublicKey v_SIZE) (slice u8) =
+let impl (#size: usize) : Core.Convert.t_From (t_KyberPublicKey v_SIZE) (array u8 v_SIZE) =
   {
-    f_impl_30__Error = Core.Array.t_TryFromSliceError;
-    f_impl_30__try_from
+    from
     =
-    fun (#v_SIZE: usize) (value: slice u8) ->
+    fun (#size: usize) (value: array u8 v_SIZE) ->
+      { Libcrux.Kem.Kyber.KyberPublicKey.f_value = value }
+  }
+
+let impl (#size: usize) : Core.Convert.t_From (array u8 v_SIZE) (t_KyberPublicKey v_SIZE) =
+  {
+    from
+    =
+    fun (#size: usize) (value: t_KyberPublicKey v_SIZE) ->
+      value.Libcrux.Kem.Kyber.KyberPublicKey.f_value
+  }
+
+let impl (#size: usize) : Core.Convert.t_TryFrom (t_KyberPublicKey v_SIZE) (slice u8) =
+  {
+    error = Core.Array.t_TryFromSliceError;
+    try_from
+    =
+    fun (#size: usize) (value: slice u8) ->
       Rust_primitives.Hax.Control_flow_monad.Mexception.run (let* hoist15:array u8 v_SIZE =
             match
-              Core.Ops.Try_trait.f_branch (Core.Convert.f_try_into value
+              Core.Ops.Try_trait.Try.branch (Core.Convert.TryInto.try_into value
                   <:
-                  Core.Result.t_Result (array u8 v_SIZE) _.f_Error)
+                  Core.Result.t_Result (array u8 v_SIZE) _)
             with
-            | Core.Ops.Control_flow.ControlFlow_Break
-              { Core.Ops.Control_flow.ControlFlow._0 = residual } ->
+            | Core.Ops.Control_flow.ControlFlow_Break residual ->
               let* hoist14:Rust_primitives.Hax.t_Never =
-                Core.Ops.Control_flow.ControlFlow.v_Break (Core.Ops.Try_trait.f_from_residual residual
-
+                Core.Ops.Control_flow.ControlFlow.v_Break (Core.Ops.Try_trait.FromResidual.from_residual
+                      residual
                     <:
                     Core.Result.t_Result (t_KyberPublicKey v_SIZE) Core.Array.t_TryFromSliceError)
               in
               Core.Ops.Control_flow.ControlFlow_Continue (Rust_primitives.Hax.never_to_any hoist14)
-            | Core.Ops.Control_flow.ControlFlow_Continue
-              { Core.Ops.Control_flow.ControlFlow._0 = v_val } ->
+            | Core.Ops.Control_flow.ControlFlow_Continue v_val ->
               Core.Ops.Control_flow.ControlFlow_Continue v_val
           in
           Core.Ops.Control_flow.ControlFlow_Continue
-          (let hoist16:t_KyberPublicKey v_SIZE = { f_value = hoist15 } in
+          (let hoist16:t_KyberPublicKey v_SIZE =
+              { Libcrux.Kem.Kyber.KyberPublicKey.f_value = hoist15 }
+            in
             Core.Result.Result_Ok hoist16))
   }
 
-let impl_31 (#v_SIZE: usize) : Core.Ops.Index.t_Index (t_KyberPublicKey v_SIZE) usize =
+let impl (#size: usize) : Core.Ops.Index.t_Index (t_KyberPublicKey v_SIZE) usize =
   {
-    f_impl_31__Output = u8;
-    f_impl_31__index
+    output = u8;
+    index
     =
-    fun (#v_SIZE: usize) (self: t_KyberPublicKey v_SIZE) (index: usize) -> self.f_value.[ index ]
+    fun (#size: usize) (self: t_KyberPublicKey v_SIZE) (index: usize) ->
+      self.Libcrux.Kem.Kyber.KyberPublicKey.f_value.[ index ]
   }
 
-let impl_32 (#v_SIZE: usize)
+let impl (#size: usize)
     : Core.Ops.Index.t_Index (t_KyberPublicKey v_SIZE) (Core.Ops.Range.t_Range usize) =
   {
-    f_impl_32__Output = slice u8;
-    f_impl_32__index
+    output = slice u8;
+    index
     =
-    fun (#v_SIZE: usize) (self: t_KyberPublicKey v_SIZE) (range: Core.Ops.Range.t_Range usize) ->
-      self.f_value.[ range ]
+    fun (#size: usize) (self: t_KyberPublicKey v_SIZE) (range: Core.Ops.Range.t_Range usize) ->
+      self.Libcrux.Kem.Kyber.KyberPublicKey.f_value.[ range ]
   }
 
-let impl_33 (#v_SIZE: usize)
+let impl (#size: usize)
     : Core.Ops.Index.t_Index (t_KyberPublicKey v_SIZE) (Core.Ops.Range.t_RangeTo usize) =
   {
-    f_impl_33__Output = slice u8;
-    f_impl_33__index
+    output = slice u8;
+    index
     =
-    fun (#v_SIZE: usize) (self: t_KyberPublicKey v_SIZE) (range: Core.Ops.Range.t_RangeTo usize) ->
-      self.f_value.[ range ]
+    fun (#size: usize) (self: t_KyberPublicKey v_SIZE) (range: Core.Ops.Range.t_RangeTo usize) ->
+      self.Libcrux.Kem.Kyber.KyberPublicKey.f_value.[ range ]
   }
 
-let impl_34 (#v_SIZE: usize)
+let impl (#size: usize)
     : Core.Ops.Index.t_Index (t_KyberPublicKey v_SIZE) (Core.Ops.Range.t_RangeFrom usize) =
   {
-    f_impl_34__Output = slice u8;
-    f_impl_34__index
+    output = slice u8;
+    index
     =
-    fun
-      (#v_SIZE: usize)
-      (self: t_KyberPublicKey v_SIZE)
-      (range: Core.Ops.Range.t_RangeFrom usize)
-      ->
-      self.f_value.[ range ]
+    fun (#size: usize) (self: t_KyberPublicKey v_SIZE) (range: Core.Ops.Range.t_RangeFrom usize) ->
+      self.Libcrux.Kem.Kyber.KyberPublicKey.f_value.[ range ]
   }
 
-let impl_35__as_slice (#v_SIZE: usize) (self: t_KyberPublicKey v_SIZE) : array u8 v_SIZE =
-  self.f_value
+let as_slice_under_impl_35 (#size: usize) (self: t_KyberPublicKey v_SIZE) : array u8 v_SIZE =
+  self.Libcrux.Kem.Kyber.KyberPublicKey.f_value
 
-let impl_35__split_at (#v_SIZE: usize) (self: t_KyberPublicKey v_SIZE) (mid: usize)
+let split_at_under_impl_35 (#size: usize) (self: t_KyberPublicKey v_SIZE) (mid: usize)
     : (slice u8 & slice u8) =
-  Core.Slice.impl__split_at (Rust_primitives.unsize self.f_value <: slice u8) mid
+  Core.Slice.split_at_under_impl (Rust_primitives.unsize self
+          .Libcrux.Kem.Kyber.KyberPublicKey.f_value
+      <:
+      slice u8)
+    mid
 
-let impl_35__len (#v_SIZE: usize) (self: t_KyberPublicKey v_SIZE) : usize = v_SIZE
+let len_under_impl_35 (#size: usize) (self: t_KyberPublicKey v_SIZE) : usize = v_SIZE
 
-type t_KyberKeyPair (#v_PRIVATE_KEY_SIZE: usize) (#v_PUBLIC_KEY_SIZE: usize) = {
+type t_KyberKeyPair = {
   f_sk:t_KyberPrivateKey v_PRIVATE_KEY_SIZE;
   f_pk:t_KyberPublicKey v_PUBLIC_KEY_SIZE
 }
@@ -400,24 +448,26 @@ type t_BadRejectionSamplingRandomnessError =
   | BadRejectionSamplingRandomnessError : t_BadRejectionSamplingRandomnessError
 
 let v_KEY_GENERATION_SEED_SIZE: usize =
-  Libcrux.Kem.Kyber.Constants.v_CPA_PKE_KEY_GENERATION_SEED_SIZE +!
+  Libcrux.Kem.Kyber.Constants.v_CPA_PKE_KEY_GENERATION_SEED_SIZE +.
   Libcrux.Kem.Kyber.Constants.v_SHARED_SECRET_SIZE
 
 let generate_keypair
-      (#v_K #v_CPA_PRIVATE_KEY_SIZE #v_PRIVATE_KEY_SIZE #v_PUBLIC_KEY_SIZE #v_BYTES_PER_RING_ELEMENT:
+      (#k #cpa_private_key_size #private_key_size #public_key_size #bytes_per_ring_element #eta1 #eta1_randomness_size:
           usize)
-      (randomness: array u8 (sz 64))
+      (randomness: array u8 64sz)
     : Core.Result.t_Result (t_KyberKeyPair v_PRIVATE_KEY_SIZE v_PUBLIC_KEY_SIZE)
       t_BadRejectionSamplingRandomnessError =
   let ind_cpa_keypair_randomness:slice u8 =
     randomness.[ {
-        Core.Ops.Range.f_start = sz 0;
-        Core.Ops.Range.f_end = Libcrux.Kem.Kyber.Constants.v_CPA_PKE_KEY_GENERATION_SEED_SIZE
+        Core.Ops.Range.Range.f_start = 0sz;
+        Core.Ops.Range.Range.f_end = Libcrux.Kem.Kyber.Constants.v_CPA_PKE_KEY_GENERATION_SEED_SIZE
       } ]
   in
   let implicit_rejection_value:slice u8 =
     randomness.[ {
-        Core.Ops.Range.f_start = Libcrux.Kem.Kyber.Constants.v_CPA_PKE_KEY_GENERATION_SEED_SIZE
+        Core.Ops.Range.RangeFrom.f_start
+        =
+        Libcrux.Kem.Kyber.Constants.v_CPA_PKE_KEY_GENERATION_SEED_SIZE
       } ]
   in
   let (ind_cpa_private_key, public_key), sampling_a_error:((Libcrux.Kem.Kyber.Ind_cpa.t_PrivateKey
@@ -427,70 +477,70 @@ let generate_keypair
     Libcrux.Kem.Kyber.Ind_cpa.generate_keypair ind_cpa_keypair_randomness
   in
   let secret_key_serialized:array u8 v_PRIVATE_KEY_SIZE =
-    Libcrux.Kem.Kyber.Ind_cpa.serialize_secret_key (Rust_primitives.unsize (Libcrux.Kem.Kyber.Ind_cpa.impl_8__as_slice
+    Libcrux.Kem.Kyber.Ind_cpa.serialize_secret_key (Rust_primitives.unsize (Libcrux.Kem.Kyber.Ind_cpa.as_slice_under_impl_8
               ind_cpa_private_key
             <:
             array u8 v_CPA_PRIVATE_KEY_SIZE)
         <:
         slice u8)
-      (Rust_primitives.unsize (impl_35__as_slice public_key <: array u8 v_PUBLIC_KEY_SIZE)
+      (Rust_primitives.unsize (as_slice_under_impl_35 public_key <: array u8 v_PUBLIC_KEY_SIZE)
         <:
         slice u8)
       implicit_rejection_value
   in
   match sampling_a_error with
-  | Core.Option.Option_Some { Core.Option.Option._0 = error } -> Core.Result.Result_Err error
+  | Core.Option.Option_Some error -> Core.Result.Result_Err error
   | _ ->
     let (private_key: t_KyberPrivateKey v_PRIVATE_KEY_SIZE):t_KyberPrivateKey v_PRIVATE_KEY_SIZE =
-      Core.Convert.f_from secret_key_serialized
+      Core.Convert.From.from secret_key_serialized
     in
-    Core.Result.Result_Ok (Libcrux.Kem.Kyber.Types.impl__from private_key public_key)
+    Core.Result.Result_Ok (Libcrux.Kem.Kyber.Types.from_under_impl private_key public_key)
 
 let encapsulate
-      (#v_K #v_SHARED_SECRET_SIZE #v_CIPHERTEXT_SIZE #v_PUBLIC_KEY_SIZE #v_T_AS_NTT_ENCODED_SIZE #v_C1_SIZE #v_C2_SIZE #v_VECTOR_U_COMPRESSION_FACTOR #v_VECTOR_V_COMPRESSION_FACTOR #v_VECTOR_U_BLOCK_LEN:
+      (#k #shared_secret_size #ciphertext_size #public_key_size #t__as_ntt_encoded_size #c1_size #c2_size #vector_u_compression_factor #vector_v_compression_factor #vector_u_block_len #eta1 #eta1_randomness_size #eta2 #eta2_randomness_size:
           usize)
       (public_key: t_KyberPublicKey v_PUBLIC_KEY_SIZE)
       (randomness: array u8 v_SHARED_SECRET_SIZE)
     : Core.Result.t_Result
       (t_KyberCiphertext v_CIPHERTEXT_SIZE & t_KyberSharedSecret v_SHARED_SECRET_SIZE)
       t_BadRejectionSamplingRandomnessError =
-  let randomness_hashed:array u8 (sz 32) =
+  let randomness_hashed:array u8 32sz =
     Libcrux.Kem.Kyber.Hash_functions.v_H (Rust_primitives.unsize randomness <: slice u8)
   in
-  let (to_hash: array u8 (sz 64)):array u8 (sz 64) =
+  let (to_hash: array u8 64sz):array u8 64sz =
     Libcrux.Kem.Kyber.Conversions.into_padded_array (Rust_primitives.unsize randomness_hashed
         <:
         slice u8)
   in
-  let to_hash:array u8 (sz 64) =
+  let to_hash:array u8 64sz =
     Rust_primitives.Hax.update_at to_hash
-      ({ Core.Ops.Range.f_start = Libcrux.Kem.Kyber.Constants.v_H_DIGEST_SIZE })
-      (Core.Slice.impl__copy_from_slice (Core.Ops.Index.IndexMut.index_mut to_hash
-              ({ Core.Ops.Range.f_start = Libcrux.Kem.Kyber.Constants.v_H_DIGEST_SIZE })
+      ({ Core.Ops.Range.RangeFrom.f_start = Libcrux.Kem.Kyber.Constants.v_H_DIGEST_SIZE })
+      (Core.Slice.copy_from_slice_under_impl (Core.Ops.Index.IndexMut.index_mut to_hash
+              ({ Core.Ops.Range.RangeFrom.f_start = Libcrux.Kem.Kyber.Constants.v_H_DIGEST_SIZE })
             <:
             slice u8)
-          (Rust_primitives.unsize (Libcrux.Kem.Kyber.Hash_functions.v_H (Rust_primitives.unsize (impl_35__as_slice
+          (Rust_primitives.unsize (Libcrux.Kem.Kyber.Hash_functions.v_H (Rust_primitives.unsize (as_slice_under_impl_35
                           public_key
                         <:
                         array u8 v_PUBLIC_KEY_SIZE)
                     <:
                     slice u8)
                 <:
-                array u8 (sz 32))
+                array u8 32sz)
             <:
             slice u8)
         <:
         slice u8)
   in
-  let hashed:array u8 (sz 64) =
+  let hashed:array u8 64sz =
     Libcrux.Kem.Kyber.Hash_functions.v_G (Rust_primitives.unsize to_hash <: slice u8)
   in
   let k_not, pseudorandomness:(slice u8 & slice u8) =
-    Core.Slice.impl__split_at (Rust_primitives.unsize hashed <: slice u8) (sz 32)
+    Core.Slice.split_at_under_impl (Rust_primitives.unsize hashed <: slice u8) 32sz
   in
   let ciphertext, sampling_a_error:(t_KyberCiphertext v_CIPHERTEXT_SIZE &
     Core.Option.t_Option t_BadRejectionSamplingRandomnessError) =
-    Libcrux.Kem.Kyber.Ind_cpa.encrypt (Rust_primitives.unsize (impl_35__as_slice public_key
+    Libcrux.Kem.Kyber.Ind_cpa.encrypt (Rust_primitives.unsize (as_slice_under_impl_35 public_key
             <:
             array u8 v_PUBLIC_KEY_SIZE)
         <:
@@ -498,108 +548,114 @@ let encapsulate
       randomness_hashed
       pseudorandomness
   in
-  let (to_hash: array u8 (sz 64)):array u8 (sz 64) =
+  let (to_hash: array u8 64sz):array u8 64sz =
     Libcrux.Kem.Kyber.Conversions.into_padded_array k_not
   in
-  let to_hash:array u8 (sz 64) =
+  let to_hash:array u8 64sz =
     Rust_primitives.Hax.update_at to_hash
-      ({ Core.Ops.Range.f_start = Libcrux.Kem.Kyber.Constants.v_H_DIGEST_SIZE })
-      (Core.Slice.impl__copy_from_slice (Core.Ops.Index.IndexMut.index_mut to_hash
-              ({ Core.Ops.Range.f_start = Libcrux.Kem.Kyber.Constants.v_H_DIGEST_SIZE })
+      ({ Core.Ops.Range.RangeFrom.f_start = Libcrux.Kem.Kyber.Constants.v_H_DIGEST_SIZE })
+      (Core.Slice.copy_from_slice_under_impl (Core.Ops.Index.IndexMut.index_mut to_hash
+              ({ Core.Ops.Range.RangeFrom.f_start = Libcrux.Kem.Kyber.Constants.v_H_DIGEST_SIZE })
             <:
             slice u8)
-          (Rust_primitives.unsize (Libcrux.Kem.Kyber.Hash_functions.v_H (Core.Convert.f_as_ref ciphertext
+          (Rust_primitives.unsize (Libcrux.Kem.Kyber.Hash_functions.v_H (Core.Convert.AsRef.as_ref ciphertext
 
                     <:
                     slice u8)
                 <:
-                array u8 (sz 32))
+                array u8 32sz)
             <:
             slice u8)
         <:
         slice u8)
   in
   let shared_secret:t_KyberSharedSecret v_SHARED_SECRET_SIZE =
-    Core.Convert.f_into (Libcrux.Kem.Kyber.Hash_functions.v_KDF (Rust_primitives.unsize to_hash
+    Core.Convert.Into.into (Libcrux.Kem.Kyber.Hash_functions.v_KDF (Rust_primitives.unsize to_hash
             <:
             slice u8)
         <:
         array u8 v_SHARED_SECRET_SIZE)
   in
-  if Core.Option.impl__is_some sampling_a_error
-  then Core.Result.Result_Err (Core.Option.impl__unwrap sampling_a_error)
+  if Core.Option.is_some_under_impl sampling_a_error
+  then Core.Result.Result_Err (Core.Option.unwrap_under_impl sampling_a_error)
   else Core.Result.Result_Ok (ciphertext, shared_secret)
 
 let decapsulate
-      (#v_K #v_SECRET_KEY_SIZE #v_CPA_SECRET_KEY_SIZE #v_PUBLIC_KEY_SIZE #v_CIPHERTEXT_SIZE #v_T_AS_NTT_ENCODED_SIZE #v_C1_SIZE #v_C2_SIZE #v_VECTOR_U_COMPRESSION_FACTOR #v_VECTOR_V_COMPRESSION_FACTOR #v_C1_BLOCK_SIZE:
+      (#k #secret_key_size #cpa_secret_key_size #public_key_size #ciphertext_size #t__as_ntt_encoded_size #c1_size #c2_size #vector_u_compression_factor #vector_v_compression_factor #c1_block_size #eta1 #eta1_randomness_size #eta2 #eta2_randomness_size:
           usize)
       (secret_key: t_KyberPrivateKey v_SECRET_KEY_SIZE)
       (ciphertext: t_KyberCiphertext v_CIPHERTEXT_SIZE)
-    : array u8 (sz 32) =
+    : array u8 32sz =
   let ind_cpa_secret_key, secret_key:(slice u8 & slice u8) =
-    impl_26__split_at secret_key v_CPA_SECRET_KEY_SIZE
+    split_at_under_impl_26 secret_key v_CPA_SECRET_KEY_SIZE
   in
   let ind_cpa_public_key, secret_key:(slice u8 & slice u8) =
-    Core.Slice.impl__split_at secret_key v_PUBLIC_KEY_SIZE
+    Core.Slice.split_at_under_impl secret_key v_PUBLIC_KEY_SIZE
   in
   let ind_cpa_public_key_hash, implicit_rejection_value:(slice u8 & slice u8) =
-    Core.Slice.impl__split_at secret_key Libcrux.Kem.Kyber.Constants.v_H_DIGEST_SIZE
+    Core.Slice.split_at_under_impl secret_key Libcrux.Kem.Kyber.Constants.v_H_DIGEST_SIZE
   in
-  let decrypted:array u8 (sz 32) =
-    Libcrux.Kem.Kyber.Ind_cpa.decrypt ind_cpa_secret_key ciphertext
-  in
-  let (to_hash: array u8 (sz 64)):array u8 (sz 64) =
+  let decrypted:array u8 32sz = Libcrux.Kem.Kyber.Ind_cpa.decrypt ind_cpa_secret_key ciphertext in
+  let (to_hash: array u8 64sz):array u8 64sz =
     Libcrux.Kem.Kyber.Conversions.into_padded_array (Rust_primitives.unsize decrypted <: slice u8)
   in
-  let to_hash:array u8 (sz 64) =
+  let to_hash:array u8 64sz =
     Rust_primitives.Hax.update_at to_hash
-      ({ Core.Ops.Range.f_start = Libcrux.Kem.Kyber.Constants.v_SHARED_SECRET_SIZE })
-      (Core.Slice.impl__copy_from_slice (Core.Ops.Index.IndexMut.index_mut to_hash
-              ({ Core.Ops.Range.f_start = Libcrux.Kem.Kyber.Constants.v_SHARED_SECRET_SIZE })
+      ({ Core.Ops.Range.RangeFrom.f_start = Libcrux.Kem.Kyber.Constants.v_SHARED_SECRET_SIZE })
+      (Core.Slice.copy_from_slice_under_impl (Core.Ops.Index.IndexMut.index_mut to_hash
+              ({
+                  Core.Ops.Range.RangeFrom.f_start
+                  =
+                  Libcrux.Kem.Kyber.Constants.v_SHARED_SECRET_SIZE
+                })
             <:
             slice u8)
           ind_cpa_public_key_hash
         <:
         slice u8)
   in
-  let hashed:array u8 (sz 64) =
+  let hashed:array u8 64sz =
     Libcrux.Kem.Kyber.Hash_functions.v_G (Rust_primitives.unsize to_hash <: slice u8)
   in
   let k_not, pseudorandomness:(slice u8 & slice u8) =
-    Core.Slice.impl__split_at (Rust_primitives.unsize hashed <: slice u8) (sz 32)
+    Core.Slice.split_at_under_impl (Rust_primitives.unsize hashed <: slice u8) 32sz
   in
   let expected_ciphertext, _:(t_KyberCiphertext v_CIPHERTEXT_SIZE &
     Core.Option.t_Option t_BadRejectionSamplingRandomnessError) =
     Libcrux.Kem.Kyber.Ind_cpa.encrypt ind_cpa_public_key decrypted pseudorandomness
   in
   let selector:u8 =
-    Libcrux.Kem.Kyber.Constant_time_ops.compare_ciphertexts_in_constant_time (Core.Convert.f_as_ref ciphertext
-
+    Libcrux.Kem.Kyber.Constant_time_ops.compare_ciphertexts_in_constant_time (Core.Convert.AsRef.as_ref
+          ciphertext
         <:
         slice u8)
-      (Core.Convert.f_as_ref expected_ciphertext <: slice u8)
+      (Core.Convert.AsRef.as_ref expected_ciphertext <: slice u8)
   in
-  let to_hash:array u8 (sz 32) =
+  let to_hash:array u8 32sz =
     Libcrux.Kem.Kyber.Constant_time_ops.select_shared_secret_in_constant_time k_not
       implicit_rejection_value
       selector
   in
-  let (to_hash: array u8 (sz 64)):array u8 (sz 64) =
+  let (to_hash: array u8 64sz):array u8 64sz =
     Libcrux.Kem.Kyber.Conversions.into_padded_array (Rust_primitives.unsize to_hash <: slice u8)
   in
-  let to_hash:array u8 (sz 64) =
+  let to_hash:array u8 64sz =
     Rust_primitives.Hax.update_at to_hash
-      ({ Core.Ops.Range.f_start = Libcrux.Kem.Kyber.Constants.v_SHARED_SECRET_SIZE })
-      (Core.Slice.impl__copy_from_slice (Core.Ops.Index.IndexMut.index_mut to_hash
-              ({ Core.Ops.Range.f_start = Libcrux.Kem.Kyber.Constants.v_SHARED_SECRET_SIZE })
+      ({ Core.Ops.Range.RangeFrom.f_start = Libcrux.Kem.Kyber.Constants.v_SHARED_SECRET_SIZE })
+      (Core.Slice.copy_from_slice_under_impl (Core.Ops.Index.IndexMut.index_mut to_hash
+              ({
+                  Core.Ops.Range.RangeFrom.f_start
+                  =
+                  Libcrux.Kem.Kyber.Constants.v_SHARED_SECRET_SIZE
+                })
             <:
             slice u8)
-          (Rust_primitives.unsize (Libcrux.Kem.Kyber.Hash_functions.v_H (Core.Convert.f_as_ref ciphertext
+          (Rust_primitives.unsize (Libcrux.Kem.Kyber.Hash_functions.v_H (Core.Convert.AsRef.as_ref ciphertext
 
                     <:
                     slice u8)
                 <:
-                array u8 (sz 32))
+                array u8 32sz)
             <:
             slice u8)
         <:
