proofs/fstar/extraction/Libcrux.Kem.Kyber.Compress.fst
@@ -3,15 +3,16 @@ module Libcrux.Kem.Kyber.Compress
 open Core
 
 let compress
-      (#v_COEFFICIENT_BITS: usize)
+      (#coefficient_bits: usize)
       (re: Libcrux.Kem.Kyber.Arithmetic.t_KyberPolynomialRingElement)
     : Libcrux.Kem.Kyber.Arithmetic.t_KyberPolynomialRingElement =
   let re:Libcrux.Kem.Kyber.Arithmetic.t_KyberPolynomialRingElement =
     {
       re with
-      Libcrux.Kem.Kyber.Arithmetic.f_coefficients
+      Libcrux.Kem.Kyber.Arithmetic.KyberPolynomialRingElement.f_coefficients
       =
-      Core.Array.impl_23__map re.Libcrux.Kem.Kyber.Arithmetic.f_coefficients
+      Core.Array.map_under_impl_23 re
+          .Libcrux.Kem.Kyber.Arithmetic.KyberPolynomialRingElement.f_coefficients
         (fun coefficient ->
             compress_q (Libcrux.Kem.Kyber.Conversions.to_unsigned_representative coefficient <: u16)
             <:
@@ -27,15 +28,16 @@ let decompress
   let re:Libcrux.Kem.Kyber.Arithmetic.t_KyberPolynomialRingElement =
     {
       re with
-      Libcrux.Kem.Kyber.Arithmetic.f_coefficients
+      Libcrux.Kem.Kyber.Arithmetic.KyberPolynomialRingElement.f_coefficients
       =
-      Core.Array.impl_23__map re.Libcrux.Kem.Kyber.Arithmetic.f_coefficients
+      Core.Array.map_under_impl_23 re
+          .Libcrux.Kem.Kyber.Arithmetic.KyberPolynomialRingElement.f_coefficients
         (fun coefficient -> decompress_q coefficient bits_per_compressed_coefficient <: i32)
     }
   in
   re
 
-let compress_q (#v_COEFFICIENT_BITS: usize) (fe: u16) : i32 =
+let compress_q (#coefficient_bits: usize) (fe: u16) : i32 =
   let _:Prims.unit =
     if true
     then
@@ -49,15 +51,13 @@ let compress_q (#v_COEFFICIENT_BITS: usize) (fe: u16) : i32 =
       in
       ()
   in
-  let two_pow_bit_size:u32 = 1ul <<! v_COEFFICIENT_BITS in
-  let compressed:u32 = (cast fe <: u32) *! (two_pow_bit_size <<! 1l <: u32) in
+  let two_pow_bit_size:u32 = 1ul >>. v_COEFFICIENT_BITS in
+  let compressed:u32 = cast fe *. (two_pow_bit_size >>. 1l <: u32) in
+  let compressed:Prims.unit = compressed +. cast Libcrux.Kem.Kyber.Constants.v_FIELD_MODULUS in
   let compressed:Prims.unit =
-    compressed +! (cast Libcrux.Kem.Kyber.Constants.v_FIELD_MODULUS <: u32)
+    compressed /. cast (Libcrux.Kem.Kyber.Constants.v_FIELD_MODULUS >>. 1l <: i32)
   in
-  let compressed:Prims.unit =
-    compressed /! (cast (Libcrux.Kem.Kyber.Constants.v_FIELD_MODULUS <<! 1l <: i32) <: u32)
-  in
-  cast (compressed &. (two_pow_bit_size -! 1ul <: u32)) <: i32
+  cast (compressed &. (two_pow_bit_size -. 1ul <: u32))
 
 let decompress_q (fe: i32) (to_bit_size: usize) : i32 =
   let _:Prims.unit =
@@ -73,9 +73,7 @@ let decompress_q (fe: i32) (to_bit_size: usize) : i32 =
       in
       ()
   in
-  let decompressed:u32 =
-    (cast fe <: u32) *! (cast Libcrux.Kem.Kyber.Constants.v_FIELD_MODULUS <: u32)
-  in
-  let decompressed:u32 = (decompressed <<! 1l <: u32) +! (1ul <<! to_bit_size <: u32) in
-  let decompressed:Prims.unit = decompressed >>! (to_bit_size +! sz 1 <: usize) in
-  cast decompressed <: i32
+  let decompressed:u32 = cast fe *. cast Libcrux.Kem.Kyber.Constants.v_FIELD_MODULUS in
+  let decompressed:u32 = (decompressed >>. 1l <: u32) +. (1ul >>. to_bit_size <: u32) in
+  let decompressed:Prims.unit = decompressed <<. (to_bit_size +. 1sz <: usize) in
+  cast decompressed
