proofs/fstar/extraction/Libcrux.Kem.Kyber.Constants.fst
@@ -4,18 +4,18 @@ open Core
 
 let v_FIELD_MODULUS: i32 = 3329l
 
-let v_BITS_PER_COEFFICIENT: usize = sz 12
+let v_BITS_PER_COEFFICIENT: usize = 12sz
 
-let v_COEFFICIENTS_IN_RING_ELEMENT: usize = sz 256
+let v_COEFFICIENTS_IN_RING_ELEMENT: usize = 256sz
 
-let v_BITS_PER_RING_ELEMENT: usize = v_COEFFICIENTS_IN_RING_ELEMENT *! sz 12
+let v_BITS_PER_RING_ELEMENT: usize = v_COEFFICIENTS_IN_RING_ELEMENT *. 12sz
 
-let v_BYTES_PER_RING_ELEMENT: usize = v_BITS_PER_RING_ELEMENT /! sz 8
+let v_BYTES_PER_RING_ELEMENT: usize = v_BITS_PER_RING_ELEMENT /. 8sz
 
-let v_REJECTION_SAMPLING_SEED_SIZE: usize = sz 168 *! sz 5
+let v_REJECTION_SAMPLING_SEED_SIZE: usize = 168sz *. 5sz
 
-let v_SHARED_SECRET_SIZE: usize = sz 32
+let v_SHARED_SECRET_SIZE: usize = 32sz
 
-let v_CPA_PKE_KEY_GENERATION_SEED_SIZE: usize = sz 32
+let v_CPA_PKE_KEY_GENERATION_SEED_SIZE: usize = 32sz
 
 let v_H_DIGEST_SIZE: usize = Libcrux.Digest.digest_size Libcrux.Digest.Algorithm_Sha3_256_
