proofs/fstar/extraction/Libcrux.Kem.Kyber.Kyber512.fst
@@ -2,76 +2,84 @@ module Libcrux.Kem.Kyber.Kyber512
 #set-options "--fuel 0 --ifuel 1 --z3rlimit 15"
 open Core
 
-let v_RANK_512_: usize = sz 2
+let v_RANK_512_: usize = 2sz
 
 let v_RANKED_BYTES_PER_RING_ELEMENT_512_: usize =
-  (v_RANK_512_ *! Libcrux.Kem.Kyber.Constants.v_BITS_PER_RING_ELEMENT <: usize) /! sz 8
+  (v_RANK_512_ *. Libcrux.Kem.Kyber.Constants.v_BITS_PER_RING_ELEMENT <: usize) /. 8sz
 
 let v_T_AS_NTT_ENCODED_SIZE_512_: usize =
-  ((v_RANK_512_ *! Libcrux.Kem.Kyber.Constants.v_COEFFICIENTS_IN_RING_ELEMENT <: usize) *!
+  ((v_RANK_512_ *. Libcrux.Kem.Kyber.Constants.v_COEFFICIENTS_IN_RING_ELEMENT <: usize) *.
     Libcrux.Kem.Kyber.Constants.v_BITS_PER_COEFFICIENT
     <:
-    usize) /!
-  sz 8
+    usize) /.
+  8sz
 
-let v_VECTOR_U_COMPRESSION_FACTOR_512_: usize = sz 10
+let v_VECTOR_U_COMPRESSION_FACTOR_512_: usize = 10sz
 
 let v_C1_BLOCK_SIZE_512_: usize =
-  (Libcrux.Kem.Kyber.Constants.v_COEFFICIENTS_IN_RING_ELEMENT *! v_VECTOR_U_COMPRESSION_FACTOR_512_
+  (Libcrux.Kem.Kyber.Constants.v_COEFFICIENTS_IN_RING_ELEMENT *. v_VECTOR_U_COMPRESSION_FACTOR_512_
     <:
-    usize) /!
-  sz 8
+    usize) /.
+  8sz
 
-let v_C1_SIZE_512_: usize = v_C1_BLOCK_SIZE_512_ *! v_RANK_512_
+let v_C1_SIZE_512_: usize = v_C1_BLOCK_SIZE_512_ *. v_RANK_512_
 
-let v_VECTOR_V_COMPRESSION_FACTOR_512_: usize = sz 4
+let v_VECTOR_V_COMPRESSION_FACTOR_512_: usize = 4sz
 
 let v_C2_SIZE_512_: usize =
-  (Libcrux.Kem.Kyber.Constants.v_COEFFICIENTS_IN_RING_ELEMENT *! v_VECTOR_V_COMPRESSION_FACTOR_512_
+  (Libcrux.Kem.Kyber.Constants.v_COEFFICIENTS_IN_RING_ELEMENT *. v_VECTOR_V_COMPRESSION_FACTOR_512_
     <:
-    usize) /!
-  sz 8
+    usize) /.
+  8sz
 
 let v_CPA_PKE_SECRET_KEY_SIZE_512_: usize =
-  ((v_RANK_512_ *! Libcrux.Kem.Kyber.Constants.v_COEFFICIENTS_IN_RING_ELEMENT <: usize) *!
+  ((v_RANK_512_ *. Libcrux.Kem.Kyber.Constants.v_COEFFICIENTS_IN_RING_ELEMENT <: usize) *.
     Libcrux.Kem.Kyber.Constants.v_BITS_PER_COEFFICIENT
     <:
-    usize) /!
-  sz 8
+    usize) /.
+  8sz
 
-let v_CPA_PKE_PUBLIC_KEY_SIZE_512_: usize = v_T_AS_NTT_ENCODED_SIZE_512_ +! sz 32
+let v_CPA_PKE_PUBLIC_KEY_SIZE_512_: usize = v_T_AS_NTT_ENCODED_SIZE_512_ +. 32sz
 
-let v_CPA_PKE_CIPHERTEXT_SIZE_512_: usize = v_C1_SIZE_512_ +! v_C2_SIZE_512_
+let v_CPA_PKE_CIPHERTEXT_SIZE_512_: usize = v_C1_SIZE_512_ +. v_C2_SIZE_512_
 
 let v_SECRET_KEY_SIZE_512_: usize =
-  ((v_CPA_PKE_SECRET_KEY_SIZE_512_ +! v_CPA_PKE_PUBLIC_KEY_SIZE_512_ <: usize) +!
+  ((v_CPA_PKE_SECRET_KEY_SIZE_512_ +. v_CPA_PKE_PUBLIC_KEY_SIZE_512_ <: usize) +.
     Libcrux.Kem.Kyber.Constants.v_H_DIGEST_SIZE
     <:
-    usize) +!
+    usize) +.
   Libcrux.Kem.Kyber.Constants.v_SHARED_SECRET_SIZE
 
-let t_Kyber512Ciphertext = Libcrux.Kem.Kyber.t_KyberCiphertext (sz 768)
+let v_ETA1: usize = 3sz
 
-let t_Kyber512PrivateKey = Libcrux.Kem.Kyber.t_KyberPrivateKey (sz 1632)
+let v_ETA1_RANDOMNESS_SIZE: usize = v_ETA1 *. 64sz
 
-let t_Kyber512PublicKey = Libcrux.Kem.Kyber.t_KyberPublicKey (sz 800)
+let v_ETA2: usize = 2sz
 
-let t_Kyber512SharedSecret = Libcrux.Kem.Kyber.t_KyberSharedSecret (sz 32)
+let v_ETA2_RANDOMNESS_SIZE: usize = v_ETA2 *. 64sz
 
-let generate_key_pair_512_ (randomness: array u8 (sz 64))
-    : Core.Result.t_Result (Libcrux.Kem.Kyber.t_KyberKeyPair (sz 1632) (sz 800))
+let t_Kyber512Ciphertext = Libcrux.Kem.Kyber.t_KyberCiphertext 768sz
+
+let t_Kyber512PrivateKey = Libcrux.Kem.Kyber.t_KyberPrivateKey 1632sz
+
+let t_Kyber512PublicKey = Libcrux.Kem.Kyber.t_KyberPublicKey 800sz
+
+let t_Kyber512SharedSecret = Libcrux.Kem.Kyber.t_KyberSharedSecret 32sz
+
+let generate_key_pair_512_ (randomness: array u8 64sz)
+    : Core.Result.t_Result (Libcrux.Kem.Kyber.t_KyberKeyPair 1632sz 800sz)
       Libcrux.Kem.Kyber.t_BadRejectionSamplingRandomnessError =
   Libcrux.Kem.Kyber.generate_keypair randomness
 
 let encapsulate_512_
-      (public_key: Libcrux.Kem.Kyber.t_KyberPublicKey (sz 800))
-      (randomness: array u8 (sz 32))
+      (public_key: Libcrux.Kem.Kyber.t_KyberPublicKey 800sz)
+      (randomness: array u8 32sz)
     : Core.Result.t_Result
-      (Libcrux.Kem.Kyber.t_KyberCiphertext (sz 768) & Libcrux.Kem.Kyber.t_KyberSharedSecret (sz 32))
+      (Libcrux.Kem.Kyber.t_KyberCiphertext 768sz & Libcrux.Kem.Kyber.t_KyberSharedSecret 32sz)
       Libcrux.Kem.Kyber.t_BadRejectionSamplingRandomnessError =
   Libcrux.Kem.Kyber.encapsulate public_key randomness
 
 let decapsulate_512_
-      (secret_key: Libcrux.Kem.Kyber.t_KyberPrivateKey (sz 1632))
-      (ciphertext: Libcrux.Kem.Kyber.t_KyberCiphertext (sz 768))
-    : array u8 (sz 32) = Libcrux.Kem.Kyber.decapsulate secret_key ciphertext
+      (secret_key: Libcrux.Kem.Kyber.t_KyberPrivateKey 1632sz)
+      (ciphertext: Libcrux.Kem.Kyber.t_KyberCiphertext 768sz)
+    : array u8 32sz = Libcrux.Kem.Kyber.decapsulate secret_key ciphertext
