proofs/fstar/extraction/Libcrux.Kem.Kyber.Serialize.fst
@@ -3,7 +3,7 @@ module Libcrux.Kem.Kyber.Serialize
 open Core
 
 let serialize_little_endian
-      (#v_COMPRESSION_FACTOR #v_OUT_LEN: usize)
+      (#compression_factor #out_len: usize)
       (re: Libcrux.Kem.Kyber.Arithmetic.t_KyberPolynomialRingElement)
     : array u8 v_OUT_LEN =
   let _:Prims.unit =
@@ -11,17 +11,17 @@ let serialize_little_endian
     then
       let _:Prims.unit =
         if
-          ~.(((Libcrux.Kem.Kyber.Constants.v_COEFFICIENTS_IN_RING_ELEMENT *! v_COMPRESSION_FACTOR
+          ~.(((Libcrux.Kem.Kyber.Constants.v_COEFFICIENTS_IN_RING_ELEMENT *. v_COMPRESSION_FACTOR
                 <:
-                usize) /!
-              sz 8
+                usize) /.
+              8sz
               <:
               usize) =.
             v_OUT_LEN
             <:
             bool)
         then
-          Rust_primitives.Hax.never_to_any (Core.Panicking.panic_fmt (Core.Fmt.impl_2__new_v1 (Rust_primitives.unsize
+          Rust_primitives.Hax.never_to_any (Core.Panicking.panic_fmt (Core.Fmt.new_v1_under_impl_2 (Rust_primitives.unsize
                         (let list = [""; " != "] in
                           FStar.Pervasives.assert_norm (Prims.eq2 (List.Tot.length list) 2);
                           Rust_primitives.Hax.array_of_list list)
@@ -29,16 +29,18 @@ let serialize_little_endian
                       slice string)
                     (Rust_primitives.unsize (let list =
                             [
-                              Core.Fmt.Rt.impl_1__new_display ((Libcrux.Kem.Kyber.Constants.v_COEFFICIENTS_IN_RING_ELEMENT *!
+                              Core.Fmt.Rt.new_display_under_impl_1 ((Libcrux.Kem.Kyber.Constants.v_COEFFICIENTS_IN_RING_ELEMENT *.
                                     v_COMPRESSION_FACTOR
                                     <:
-                                    usize) /!
-                                  sz 8
+                                    usize) /.
+                                  8sz
                                   <:
                                   usize)
                               <:
                               Core.Fmt.Rt.t_Argument;
-                              Core.Fmt.Rt.impl_1__new_display v_OUT_LEN <: Core.Fmt.Rt.t_Argument
+                              Core.Fmt.Rt.new_display_under_impl_1 v_OUT_LEN
+                              <:
+                              Core.Fmt.Rt.t_Argument
                             ]
                           in
                           FStar.Pervasives.assert_norm (Prims.eq2 (List.Tot.length list) 2);
@@ -52,7 +54,7 @@ let serialize_little_endian
       in
       ()
   in
-  match cast v_COMPRESSION_FACTOR <: u32 with
+  match cast v_COMPRESSION_FACTOR with
   | 1ul -> serialize_little_endian_1_ re
   | 4ul -> serialize_little_endian_4_ re
   | 5ul -> serialize_little_endian_5_ re
@@ -60,7 +62,7 @@ let serialize_little_endian
   | 11ul -> serialize_little_endian_11_ re
   | 12ul -> serialize_little_endian_12_ re
   | _ ->
-    Rust_primitives.Hax.never_to_any (Core.Panicking.panic_fmt (Core.Fmt.impl_2__new_v1 (Rust_primitives.unsize
+    Rust_primitives.Hax.never_to_any (Core.Panicking.panic_fmt (Core.Fmt.new_v1_under_impl_2 (Rust_primitives.unsize
                   (let list = ["internal error: entered unreachable code: factor "] in
                     FStar.Pervasives.assert_norm (Prims.eq2 (List.Tot.length list) 1);
                     Rust_primitives.Hax.array_of_list list)
@@ -68,7 +70,7 @@ let serialize_little_endian
                 slice string)
               (Rust_primitives.unsize (let list =
                       [
-                        Core.Fmt.Rt.impl_1__new_display v_COMPRESSION_FACTOR
+                        Core.Fmt.Rt.new_display_under_impl_1 v_COMPRESSION_FACTOR
                         <:
                         Core.Fmt.Rt.t_Argument
                       ]
@@ -82,18 +84,18 @@ let serialize_little_endian
         <:
         Rust_primitives.Hax.t_Never)
 
-let deserialize_little_endian (#v_COMPRESSION_FACTOR: usize) (serialized: slice u8)
+let deserialize_little_endian (#compression_factor: usize) (serialized: slice u8)
     : Libcrux.Kem.Kyber.Arithmetic.t_KyberPolynomialRingElement =
   let _:Prims.unit =
     if true
     then
       let _:Prims.unit =
         match
-          Core.Slice.impl__len serialized,
-          (Libcrux.Kem.Kyber.Constants.v_COEFFICIENTS_IN_RING_ELEMENT *! v_COMPRESSION_FACTOR
+          Core.Slice.len_under_impl serialized,
+          (Libcrux.Kem.Kyber.Constants.v_COEFFICIENTS_IN_RING_ELEMENT *. v_COMPRESSION_FACTOR
             <:
-            usize) /!
-          sz 8
+            usize) /.
+          8sz
         with
         | left_val, right_val ->
           if ~.(left_val =. right_val <: bool)
@@ -108,7 +110,7 @@ let deserialize_little_endian (#v_COMPRESSION_FACTOR: usize) (serialized: slice 
       in
       ()
   in
-  match cast v_COMPRESSION_FACTOR <: u32 with
+  match cast v_COMPRESSION_FACTOR with
   | 1ul -> deserialize_little_endian_1_ serialized
   | 4ul -> deserialize_little_endian_4_ serialized
   | 5ul -> deserialize_little_endian_5_ serialized
@@ -116,7 +118,7 @@ let deserialize_little_endian (#v_COMPRESSION_FACTOR: usize) (serialized: slice 
   | 11ul -> deserialize_little_endian_11_ serialized
   | 12ul -> deserialize_little_endian_12_ serialized
   | _ ->
-    Rust_primitives.Hax.never_to_any (Core.Panicking.panic_fmt (Core.Fmt.impl_2__new_v1 (Rust_primitives.unsize
+    Rust_primitives.Hax.never_to_any (Core.Panicking.panic_fmt (Core.Fmt.new_v1_under_impl_2 (Rust_primitives.unsize
                   (let list = ["internal error: entered unreachable code: factor "] in
                     FStar.Pervasives.assert_norm (Prims.eq2 (List.Tot.length list) 1);
                     Rust_primitives.Hax.array_of_list list)
@@ -124,7 +126,7 @@ let deserialize_little_endian (#v_COMPRESSION_FACTOR: usize) (serialized: slice 
                 slice string)
               (Rust_primitives.unsize (let list =
                       [
-                        Core.Fmt.Rt.impl_1__new_display v_COMPRESSION_FACTOR
+                        Core.Fmt.Rt.new_display_under_impl_1 v_COMPRESSION_FACTOR
                         <:
                         Core.Fmt.Rt.t_Argument
                       ]
@@ -139,36 +141,36 @@ let deserialize_little_endian (#v_COMPRESSION_FACTOR: usize) (serialized: slice 
         Rust_primitives.Hax.t_Never)
 
 let serialize_little_endian_1_
-      (#v_OUT_LEN: usize)
+      (#out_len: usize)
       (re: Libcrux.Kem.Kyber.Arithmetic.t_KyberPolynomialRingElement)
     : array u8 v_OUT_LEN =
   let serialized:array u8 v_OUT_LEN = Rust_primitives.Hax.repeat 0uy v_OUT_LEN in
   let serialized:array u8 v_OUT_LEN =
-    Core.Iter.Traits.Iterator.Iterator.fold (Core.Iter.Traits.Collect.f_into_iter (Core.Iter.Traits.Iterator.f_enumerate
-              (Core.Slice.impl__chunks_exact (Rust_primitives.unsize re
-                        .Libcrux.Kem.Kyber.Arithmetic.f_coefficients
+    Core.Iter.Traits.Iterator.Iterator.fold (Core.Iter.Traits.Collect.IntoIterator.into_iter (Core.Iter.Traits.Iterator.Iterator.enumerate
+              (Core.Slice.chunks_exact_under_impl (Rust_primitives.unsize re
+                        .Libcrux.Kem.Kyber.Arithmetic.KyberPolynomialRingElement.f_coefficients
                     <:
                     slice i32)
-                  (sz 8)
+                  8sz
                 <:
                 Core.Slice.Iter.t_ChunksExact i32)
             <:
             Core.Iter.Adapters.Enumerate.t_Enumerate (Core.Slice.Iter.t_ChunksExact i32))
         <:
-        _.f_IntoIter)
+        _)
       serialized
       (fun serialized (i, chunk) ->
-          Core.Iter.Traits.Iterator.Iterator.fold (Core.Iter.Traits.Collect.f_into_iter (Core.Iter.Traits.Iterator.f_enumerate
-                    (Core.Slice.impl__iter chunk <: Core.Slice.Iter.t_Iter i32)
+          Core.Iter.Traits.Iterator.Iterator.fold (Core.Iter.Traits.Collect.IntoIterator.into_iter (Core.Iter.Traits.Iterator.Iterator.enumerate
+                    (Core.Slice.iter_under_impl chunk <: Core.Slice.Iter.t_Iter i32)
                   <:
                   Core.Iter.Adapters.Enumerate.t_Enumerate (Core.Slice.Iter.t_Iter i32))
               <:
-              _.f_IntoIter)
+              _)
             serialized
             (fun serialized (j, coefficient) ->
                 Rust_primitives.Hax.update_at serialized
                   i
-                  ((serialized.[ i ] <: u8) |. ((cast coefficient <: u8) <<! j <: u8) <: Prims.unit)
+                  ((serialized.[ i ] <: u8) |. (cast coefficient >>. j <: u8) <: Prims.unit)
                 <:
                 array u8 v_OUT_LEN)
           <:
@@ -183,8 +185,8 @@ let deserialize_little_endian_1_ (serialized: slice u8)
     then
       let _:Prims.unit =
         match
-          Core.Slice.impl__len serialized,
-          Libcrux.Kem.Kyber.Constants.v_COEFFICIENTS_IN_RING_ELEMENT /! sz 8
+          Core.Slice.len_under_impl serialized,
+          Libcrux.Kem.Kyber.Constants.v_COEFFICIENTS_IN_RING_ELEMENT /. 8sz
         with
         | left_val, right_val ->
           if ~.(left_val =. right_val <: bool)
@@ -200,32 +202,33 @@ let deserialize_little_endian_1_ (serialized: slice u8)
       ()
   in
   let re:Libcrux.Kem.Kyber.Arithmetic.t_KyberPolynomialRingElement =
-    Libcrux.Kem.Kyber.Arithmetic.impl__ZERO
+    Libcrux.Kem.Kyber.Arithmetic.v_ZERO_under_impl
   in
   let re:Libcrux.Kem.Kyber.Arithmetic.t_KyberPolynomialRingElement =
-    Core.Iter.Traits.Iterator.Iterator.fold (Core.Iter.Traits.Collect.f_into_iter (Core.Iter.Traits.Iterator.f_enumerate
-              (Core.Slice.impl__iter serialized <: Core.Slice.Iter.t_Iter u8)
+    Core.Iter.Traits.Iterator.Iterator.fold (Core.Iter.Traits.Collect.IntoIterator.into_iter (Core.Iter.Traits.Iterator.Iterator.enumerate
+              (Core.Slice.iter_under_impl serialized <: Core.Slice.Iter.t_Iter u8)
             <:
             Core.Iter.Adapters.Enumerate.t_Enumerate (Core.Slice.Iter.t_Iter u8))
         <:
-        _.f_IntoIter)
+        _)
       re
       (fun re (i, byte) ->
-          Core.Iter.Traits.Iterator.Iterator.fold (Core.Iter.Traits.Collect.f_into_iter ({
-                    Core.Ops.Range.f_start = sz 0;
-                    Core.Ops.Range.f_end = sz 8
+          Core.Iter.Traits.Iterator.Iterator.fold (Core.Iter.Traits.Collect.IntoIterator.into_iter ({
+                    Core.Ops.Range.Range.f_start = 0sz;
+                    Core.Ops.Range.Range.f_end = 8sz
                   })
               <:
-              _.f_IntoIter)
+              _)
             re
             (fun re j ->
                 {
                   re with
-                  Libcrux.Kem.Kyber.Arithmetic.f_coefficients
+                  Libcrux.Kem.Kyber.Arithmetic.KyberPolynomialRingElement.f_coefficients
                   =
-                  Rust_primitives.Hax.update_at re.Libcrux.Kem.Kyber.Arithmetic.f_coefficients
-                    ((sz 8 *! i <: usize) +! j <: usize)
-                    (cast ((byte >>! j <: (Core.Ops.Bit.t_impl_780).f_Output) &. 1uy <: u8) <: i32)
+                  Rust_primitives.Hax.update_at re
+                      .Libcrux.Kem.Kyber.Arithmetic.KyberPolynomialRingElement.f_coefficients
+                    ((8sz *. i <: usize) +. j <: usize)
+                    (cast ((byte <<. j <: _) &. 1uy <: u8))
                   <:
                   Libcrux.Kem.Kyber.Arithmetic.t_KyberPolynomialRingElement
                 })
@@ -235,31 +238,31 @@ let deserialize_little_endian_1_ (serialized: slice u8)
   re
 
 let serialize_little_endian_4_
-      (#v_OUT_LEN: usize)
+      (#out_len: usize)
       (re: Libcrux.Kem.Kyber.Arithmetic.t_KyberPolynomialRingElement)
     : array u8 v_OUT_LEN =
   let serialized:array u8 v_OUT_LEN = Rust_primitives.Hax.repeat 0uy v_OUT_LEN in
   let serialized:array u8 v_OUT_LEN =
-    Core.Iter.Traits.Iterator.Iterator.fold (Core.Iter.Traits.Collect.f_into_iter (Core.Iter.Traits.Iterator.f_enumerate
-              (Core.Slice.impl__chunks_exact (Rust_primitives.unsize re
-                        .Libcrux.Kem.Kyber.Arithmetic.f_coefficients
+    Core.Iter.Traits.Iterator.Iterator.fold (Core.Iter.Traits.Collect.IntoIterator.into_iter (Core.Iter.Traits.Iterator.Iterator.enumerate
+              (Core.Slice.chunks_exact_under_impl (Rust_primitives.unsize re
+                        .Libcrux.Kem.Kyber.Arithmetic.KyberPolynomialRingElement.f_coefficients
                     <:
                     slice i32)
-                  (sz 2)
+                  2sz
                 <:
                 Core.Slice.Iter.t_ChunksExact i32)
             <:
             Core.Iter.Adapters.Enumerate.t_Enumerate (Core.Slice.Iter.t_ChunksExact i32))
         <:
-        _.f_IntoIter)
+        _)
       serialized
       (fun serialized (i, chunk) ->
-          let coefficient1:u8 = cast chunk.[ sz 0 ] <: u8 in
-          let coefficient2:u8 = cast chunk.[ sz 1 ] <: u8 in
+          let coefficient1:u8 = cast chunk.[ 0sz ] in
+          let coefficient2:u8 = cast chunk.[ 1sz ] in
           let serialized:array u8 v_OUT_LEN =
             Rust_primitives.Hax.update_at serialized
               i
-              ((coefficient2 <<! 4l <: u8) |. coefficient1 <: u8)
+              ((coefficient2 >>. 4l <: u8) |. coefficient1 <: u8)
           in
           serialized)
   in
@@ -272,8 +275,8 @@ let deserialize_little_endian_4_ (serialized: slice u8)
     then
       let _:Prims.unit =
         match
-          Core.Slice.impl__len serialized,
-          (Libcrux.Kem.Kyber.Constants.v_COEFFICIENTS_IN_RING_ELEMENT *! sz 4 <: usize) /! sz 8
+          Core.Slice.len_under_impl serialized,
+          (Libcrux.Kem.Kyber.Constants.v_COEFFICIENTS_IN_RING_ELEMENT *. 4sz <: usize) /. 8sz
         with
         | left_val, right_val ->
           if ~.(left_val =. right_val <: bool)
@@ -289,35 +292,37 @@ let deserialize_little_endian_4_ (serialized: slice u8)
       ()
   in
   let re:Libcrux.Kem.Kyber.Arithmetic.t_KyberPolynomialRingElement =
-    Libcrux.Kem.Kyber.Arithmetic.impl__ZERO
+    Libcrux.Kem.Kyber.Arithmetic.v_ZERO_under_impl
   in
   let re:Libcrux.Kem.Kyber.Arithmetic.t_KyberPolynomialRingElement =
-    Core.Iter.Traits.Iterator.Iterator.fold (Core.Iter.Traits.Collect.f_into_iter (Core.Iter.Traits.Iterator.f_enumerate
-              (Core.Slice.impl__iter serialized <: Core.Slice.Iter.t_Iter u8)
+    Core.Iter.Traits.Iterator.Iterator.fold (Core.Iter.Traits.Collect.IntoIterator.into_iter (Core.Iter.Traits.Iterator.Iterator.enumerate
+              (Core.Slice.iter_under_impl serialized <: Core.Slice.Iter.t_Iter u8)
             <:
             Core.Iter.Adapters.Enumerate.t_Enumerate (Core.Slice.Iter.t_Iter u8))
         <:
-        _.f_IntoIter)
+        _)
       re
       (fun re (i, byte) ->
           let re:Libcrux.Kem.Kyber.Arithmetic.t_KyberPolynomialRingElement =
             {
               re with
-              Libcrux.Kem.Kyber.Arithmetic.f_coefficients
+              Libcrux.Kem.Kyber.Arithmetic.KyberPolynomialRingElement.f_coefficients
               =
-              Rust_primitives.Hax.update_at re.Libcrux.Kem.Kyber.Arithmetic.f_coefficients
-                (sz 2 *! i <: usize)
-                (cast (byte &. 15uy <: (Core.Ops.Bit.t_impl_46).f_Output) <: i32)
+              Rust_primitives.Hax.update_at re
+                  .Libcrux.Kem.Kyber.Arithmetic.KyberPolynomialRingElement.f_coefficients
+                (2sz *. i <: usize)
+                (cast (byte &. 15uy <: _))
             }
           in
           let re:Libcrux.Kem.Kyber.Arithmetic.t_KyberPolynomialRingElement =
             {
               re with
-              Libcrux.Kem.Kyber.Arithmetic.f_coefficients
+              Libcrux.Kem.Kyber.Arithmetic.KyberPolynomialRingElement.f_coefficients
               =
-              Rust_primitives.Hax.update_at re.Libcrux.Kem.Kyber.Arithmetic.f_coefficients
-                ((sz 2 *! i <: usize) +! sz 1 <: usize)
-                (cast ((byte >>! 4l <: (Core.Ops.Bit.t_impl_792).f_Output) &. 15uy <: u8) <: i32)
+              Rust_primitives.Hax.update_at re
+                  .Libcrux.Kem.Kyber.Arithmetic.KyberPolynomialRingElement.f_coefficients
+                ((2sz *. i <: usize) +. 1sz <: usize)
+                (cast ((byte <<. 4l <: _) &. 15uy <: u8))
             }
           in
           re)
@@ -325,31 +330,63 @@ let deserialize_little_endian_4_ (serialized: slice u8)
   re
 
 let serialize_little_endian_5_
-      (#v_OUT_LEN: usize)
+      (#out_len: usize)
       (re: Libcrux.Kem.Kyber.Arithmetic.t_KyberPolynomialRingElement)
     : array u8 v_OUT_LEN =
   let serialized:array u8 v_OUT_LEN = Rust_primitives.Hax.repeat 0uy v_OUT_LEN in
   let serialized:array u8 v_OUT_LEN =
-    Core.Iter.Traits.Iterator.Iterator.fold (Core.Iter.Traits.Collect.f_into_iter (Core.Iter.Traits.Iterator.f_enumerate
-              (Core.Slice.impl__chunks_exact (Rust_primitives.unsize re
-                        .Libcrux.Kem.Kyber.Arithmetic.f_coefficients
+    Core.Iter.Traits.Iterator.Iterator.fold (Core.Iter.Traits.Collect.IntoIterator.into_iter (Core.Iter.Traits.Iterator.Iterator.enumerate
+              (Core.Slice.chunks_exact_under_impl (Rust_primitives.unsize re
+                        .Libcrux.Kem.Kyber.Arithmetic.KyberPolynomialRingElement.f_coefficients
                     <:
                     slice i32)
-                  (sz 2)
+                  8sz
                 <:
                 Core.Slice.Iter.t_ChunksExact i32)
             <:
             Core.Iter.Adapters.Enumerate.t_Enumerate (Core.Slice.Iter.t_ChunksExact i32))
         <:
-        _.f_IntoIter)
+        _)
       serialized
-      (fun serialized (i, chunk) ->
-          let coefficient1:u8 = cast chunk.[ sz 0 ] <: u8 in
-          let coefficient2:u8 = cast chunk.[ sz 1 ] <: u8 in
+      (fun serialized (i, coefficients) ->
+          let coefficient1:u8 = cast coefficients.[ 0sz ] in
+          let coefficient2:u8 = cast coefficients.[ 1sz ] in
+          let coefficient3:u8 = cast coefficients.[ 2sz ] in
+          let coefficient4:u8 = cast coefficients.[ 3sz ] in
+          let coefficient5:u8 = cast coefficients.[ 4sz ] in
+          let coefficient6:u8 = cast coefficients.[ 5sz ] in
+          let coefficient7:u8 = cast coefficients.[ 6sz ] in
+          let coefficient8:u8 = cast coefficients.[ 7sz ] in
           let serialized:array u8 v_OUT_LEN =
             Rust_primitives.Hax.update_at serialized
-              i
-              ((coefficient2 <<! 4l <: u8) |. coefficient1 <: u8)
+              (5sz *. i <: usize)
+              (((coefficient2 &. 7uy <: u8) >>. 5l <: u8) |. coefficient1 <: u8)
+          in
+          let serialized:array u8 v_OUT_LEN =
+            Rust_primitives.Hax.update_at serialized
+              ((5sz *. i <: usize) +. 1sz <: usize)
+              ((((coefficient4 &. 1uy <: u8) >>. 7l <: u8) |. (coefficient3 >>. 2l <: u8) <: u8) |.
+                (coefficient2 <<. 3l <: u8)
+                <:
+                u8)
+          in
+          let serialized:array u8 v_OUT_LEN =
+            Rust_primitives.Hax.update_at serialized
+              ((5sz *. i <: usize) +. 2sz <: usize)
+              (((coefficient5 &. 15uy <: u8) >>. 4l <: u8) |. (coefficient4 <<. 1l <: u8) <: u8)
+          in
+          let serialized:array u8 v_OUT_LEN =
+            Rust_primitives.Hax.update_at serialized
+              ((5sz *. i <: usize) +. 3sz <: usize)
+              ((((coefficient7 &. 3uy <: u8) >>. 6l <: u8) |. (coefficient6 >>. 1l <: u8) <: u8) |.
+                (coefficient5 <<. 4l <: u8)
+                <:
+                u8)
+          in
+          let serialized:array u8 v_OUT_LEN =
+            Rust_primitives.Hax.update_at serialized
+              ((5sz *. i <: usize) +. 4sz <: usize)
+              ((coefficient8 >>. 3l <: u8) |. (coefficient7 <<. 2l <: u8) <: u8)
           in
           serialized)
   in
@@ -362,8 +399,8 @@ let deserialize_little_endian_5_ (serialized: slice u8)
     then
       let _:Prims.unit =
         match
-          Core.Slice.impl__len serialized,
-          (Libcrux.Kem.Kyber.Constants.v_COEFFICIENTS_IN_RING_ELEMENT *! sz 5 <: usize) /! sz 8
+          Core.Slice.len_under_impl serialized,
+          (Libcrux.Kem.Kyber.Constants.v_COEFFICIENTS_IN_RING_ELEMENT *. 5sz <: usize) /. 8sz
         with
         | left_val, right_val ->
           if ~.(left_val =. right_val <: bool)
@@ -379,35 +416,109 @@ let deserialize_little_endian_5_ (serialized: slice u8)
       ()
   in
   let re:Libcrux.Kem.Kyber.Arithmetic.t_KyberPolynomialRingElement =
-    Libcrux.Kem.Kyber.Arithmetic.impl__ZERO
+    Libcrux.Kem.Kyber.Arithmetic.v_ZERO_under_impl
   in
   let re:Libcrux.Kem.Kyber.Arithmetic.t_KyberPolynomialRingElement =
-    Core.Iter.Traits.Iterator.Iterator.fold (Core.Iter.Traits.Collect.f_into_iter (Core.Iter.Traits.Iterator.f_enumerate
-              (Core.Slice.impl__iter serialized <: Core.Slice.Iter.t_Iter u8)
+    Core.Iter.Traits.Iterator.Iterator.fold (Core.Iter.Traits.Collect.IntoIterator.into_iter (Core.Iter.Traits.Iterator.Iterator.enumerate
+              (Core.Slice.chunks_exact_under_impl serialized 5sz <: Core.Slice.Iter.t_ChunksExact u8
+              )
             <:
-            Core.Iter.Adapters.Enumerate.t_Enumerate (Core.Slice.Iter.t_Iter u8))
+            Core.Iter.Adapters.Enumerate.t_Enumerate (Core.Slice.Iter.t_ChunksExact u8))
         <:
-        _.f_IntoIter)
+        _)
       re
-      (fun re (i, byte) ->
+      (fun re (i, bytes) ->
+          let byte1:i32 = cast bytes.[ 0sz ] in
+          let byte2:i32 = cast bytes.[ 1sz ] in
+          let byte3:i32 = cast bytes.[ 2sz ] in
+          let byte4:i32 = cast bytes.[ 3sz ] in
+          let byte5:i32 = cast bytes.[ 4sz ] in
           let re:Libcrux.Kem.Kyber.Arithmetic.t_KyberPolynomialRingElement =
             {
               re with
-              Libcrux.Kem.Kyber.Arithmetic.f_coefficients
+              Libcrux.Kem.Kyber.Arithmetic.KyberPolynomialRingElement.f_coefficients
               =
-              Rust_primitives.Hax.update_at re.Libcrux.Kem.Kyber.Arithmetic.f_coefficients
-                (sz 2 *! i <: usize)
-                (cast (byte &. 15uy <: (Core.Ops.Bit.t_impl_46).f_Output) <: i32)
+              Rust_primitives.Hax.update_at re
+                  .Libcrux.Kem.Kyber.Arithmetic.KyberPolynomialRingElement.f_coefficients
+                (8sz *. i <: usize)
+                (byte1 &. 31l <: i32)
             }
           in
           let re:Libcrux.Kem.Kyber.Arithmetic.t_KyberPolynomialRingElement =
             {
               re with
-              Libcrux.Kem.Kyber.Arithmetic.f_coefficients
+              Libcrux.Kem.Kyber.Arithmetic.KyberPolynomialRingElement.f_coefficients
               =
-              Rust_primitives.Hax.update_at re.Libcrux.Kem.Kyber.Arithmetic.f_coefficients
-                ((sz 2 *! i <: usize) +! sz 1 <: usize)
-                (cast ((byte >>! 4l <: (Core.Ops.Bit.t_impl_792).f_Output) &. 15uy <: u8) <: i32)
+              Rust_primitives.Hax.update_at re
+                  .Libcrux.Kem.Kyber.Arithmetic.KyberPolynomialRingElement.f_coefficients
+                ((8sz *. i <: usize) +. 1sz <: usize)
+                (((byte2 &. 3l <: i32) >>. 3l <: i32) |. (byte1 <<. 5l <: i32) <: i32)
+            }
+          in
+          let re:Libcrux.Kem.Kyber.Arithmetic.t_KyberPolynomialRingElement =
+            {
+              re with
+              Libcrux.Kem.Kyber.Arithmetic.KyberPolynomialRingElement.f_coefficients
+              =
+              Rust_primitives.Hax.update_at re
+                  .Libcrux.Kem.Kyber.Arithmetic.KyberPolynomialRingElement.f_coefficients
+                ((8sz *. i <: usize) +. 2sz <: usize)
+                ((byte2 <<. 2l <: i32) &. 31l <: i32)
+            }
+          in
+          let re:Libcrux.Kem.Kyber.Arithmetic.t_KyberPolynomialRingElement =
+            {
+              re with
+              Libcrux.Kem.Kyber.Arithmetic.KyberPolynomialRingElement.f_coefficients
+              =
+              Rust_primitives.Hax.update_at re
+                  .Libcrux.Kem.Kyber.Arithmetic.KyberPolynomialRingElement.f_coefficients
+                ((8sz *. i <: usize) +. 3sz <: usize)
+                (((byte3 &. 15l <: i32) >>. 1l <: i32) |. (byte2 <<. 7l <: i32) <: i32)
+            }
+          in
+          let re:Libcrux.Kem.Kyber.Arithmetic.t_KyberPolynomialRingElement =
+            {
+              re with
+              Libcrux.Kem.Kyber.Arithmetic.KyberPolynomialRingElement.f_coefficients
+              =
+              Rust_primitives.Hax.update_at re
+                  .Libcrux.Kem.Kyber.Arithmetic.KyberPolynomialRingElement.f_coefficients
+                ((8sz *. i <: usize) +. 4sz <: usize)
+                (((byte4 &. 1l <: i32) >>. 4l <: i32) |. (byte3 <<. 4l <: i32) <: i32)
+            }
+          in
+          let re:Libcrux.Kem.Kyber.Arithmetic.t_KyberPolynomialRingElement =
+            {
+              re with
+              Libcrux.Kem.Kyber.Arithmetic.KyberPolynomialRingElement.f_coefficients
+              =
+              Rust_primitives.Hax.update_at re
+                  .Libcrux.Kem.Kyber.Arithmetic.KyberPolynomialRingElement.f_coefficients
+                ((8sz *. i <: usize) +. 5sz <: usize)
+                ((byte4 <<. 1l <: i32) &. 31l <: i32)
+            }
+          in
+          let re:Libcrux.Kem.Kyber.Arithmetic.t_KyberPolynomialRingElement =
+            {
+              re with
+              Libcrux.Kem.Kyber.Arithmetic.KyberPolynomialRingElement.f_coefficients
+              =
+              Rust_primitives.Hax.update_at re
+                  .Libcrux.Kem.Kyber.Arithmetic.KyberPolynomialRingElement.f_coefficients
+                ((8sz *. i <: usize) +. 6sz <: usize)
+                (((byte5 &. 7l <: i32) >>. 2l <: i32) |. (byte4 <<. 6l <: i32) <: i32)
+            }
+          in
+          let re:Libcrux.Kem.Kyber.Arithmetic.t_KyberPolynomialRingElement =
+            {
+              re with
+              Libcrux.Kem.Kyber.Arithmetic.KyberPolynomialRingElement.f_coefficients
+              =
+              Rust_primitives.Hax.update_at re
+                  .Libcrux.Kem.Kyber.Arithmetic.KyberPolynomialRingElement.f_coefficients
+                ((8sz *. i <: usize) +. 7sz <: usize)
+                (byte5 <<. 3l <: i32)
             }
           in
           re)
@@ -415,62 +526,62 @@ let deserialize_little_endian_5_ (serialized: slice u8)
   re
 
 let serialize_little_endian_10_
-      (#v_OUT_LEN: usize)
+      (#out_len: usize)
       (re: Libcrux.Kem.Kyber.Arithmetic.t_KyberPolynomialRingElement)
     : array u8 v_OUT_LEN =
   let serialized:array u8 v_OUT_LEN = Rust_primitives.Hax.repeat 0uy v_OUT_LEN in
   let serialized:array u8 v_OUT_LEN =
-    Core.Iter.Traits.Iterator.Iterator.fold (Core.Iter.Traits.Collect.f_into_iter (Core.Iter.Traits.Iterator.f_enumerate
-              (Core.Slice.impl__chunks_exact (Rust_primitives.unsize re
-                        .Libcrux.Kem.Kyber.Arithmetic.f_coefficients
+    Core.Iter.Traits.Iterator.Iterator.fold (Core.Iter.Traits.Collect.IntoIterator.into_iter (Core.Iter.Traits.Iterator.Iterator.enumerate
+              (Core.Slice.chunks_exact_under_impl (Rust_primitives.unsize re
+                        .Libcrux.Kem.Kyber.Arithmetic.KyberPolynomialRingElement.f_coefficients
                     <:
                     slice i32)
-                  (sz 4)
+                  4sz
                 <:
                 Core.Slice.Iter.t_ChunksExact i32)
             <:
             Core.Iter.Adapters.Enumerate.t_Enumerate (Core.Slice.Iter.t_ChunksExact i32))
         <:
-        _.f_IntoIter)
+        _)
       serialized
       (fun serialized (i, chunk) ->
-          let coefficient1:i32 = chunk.[ sz 0 ] in
-          let coefficient2:i32 = chunk.[ sz 1 ] in
-          let coefficient3:i32 = chunk.[ sz 2 ] in
-          let coefficient4:i32 = chunk.[ sz 3 ] in
+          let coefficient1:i32 = chunk.[ 0sz ] in
+          let coefficient2:i32 = chunk.[ 1sz ] in
+          let coefficient3:i32 = chunk.[ 2sz ] in
+          let coefficient4:i32 = chunk.[ 3sz ] in
           let serialized:array u8 v_OUT_LEN =
             Rust_primitives.Hax.update_at serialized
-              (sz 5 *! i <: usize)
-              (cast (coefficient1 &. 255l <: i32) <: u8)
+              (5sz *. i <: usize)
+              (cast (coefficient1 &. 255l <: i32))
           in
           let serialized:array u8 v_OUT_LEN =
             Rust_primitives.Hax.update_at serialized
-              ((sz 5 *! i <: usize) +! sz 1 <: usize)
-              (((cast (coefficient2 &. 63l <: i32) <: u8) <<! 2l <: u8) |.
-                (cast ((coefficient1 >>! 8l <: i32) &. 3l <: i32) <: u8)
+              ((5sz *. i <: usize) +. 1sz <: usize)
+              ((cast (coefficient2 &. 63l <: i32) >>. 2l <: u8) |.
+                cast ((coefficient1 <<. 8l <: i32) &. 3l <: i32)
                 <:
                 u8)
           in
           let serialized:array u8 v_OUT_LEN =
             Rust_primitives.Hax.update_at serialized
-              ((sz 5 *! i <: usize) +! sz 2 <: usize)
-              (((cast (coefficient3 &. 15l <: i32) <: u8) <<! 4l <: u8) |.
-                (cast ((coefficient2 >>! 6l <: i32) &. 15l <: i32) <: u8)
+              ((5sz *. i <: usize) +. 2sz <: usize)
+              ((cast (coefficient3 &. 15l <: i32) >>. 4l <: u8) |.
+                cast ((coefficient2 <<. 6l <: i32) &. 15l <: i32)
                 <:
                 u8)
           in
           let serialized:array u8 v_OUT_LEN =
             Rust_primitives.Hax.update_at serialized
-              ((sz 5 *! i <: usize) +! sz 3 <: usize)
-              (((cast (coefficient4 &. 3l <: i32) <: u8) <<! 6l <: u8) |.
-                (cast ((coefficient3 >>! 4l <: i32) &. 63l <: i32) <: u8)
+              ((5sz *. i <: usize) +. 3sz <: usize)
+              ((cast (coefficient4 &. 3l <: i32) >>. 6l <: u8) |.
+                cast ((coefficient3 <<. 4l <: i32) &. 63l <: i32)
                 <:
                 u8)
           in
           let serialized:array u8 v_OUT_LEN =
             Rust_primitives.Hax.update_at serialized
-              ((sz 5 *! i <: usize) +! sz 4 <: usize)
-              (cast ((coefficient4 >>! 2l <: i32) &. 255l <: i32) <: u8)
+              ((5sz *. i <: usize) +. 4sz <: usize)
+              (cast ((coefficient4 <<. 2l <: i32) &. 255l <: i32))
           in
           serialized)
   in
@@ -483,8 +594,8 @@ let deserialize_little_endian_10_ (serialized: slice u8)
     then
       let _:Prims.unit =
         match
-          Core.Slice.impl__len serialized,
-          (Libcrux.Kem.Kyber.Constants.v_COEFFICIENTS_IN_RING_ELEMENT *! sz 10 <: usize) /! sz 8
+          Core.Slice.len_under_impl serialized,
+          (Libcrux.Kem.Kyber.Constants.v_COEFFICIENTS_IN_RING_ELEMENT *. 10sz <: usize) /. 8sz
         with
         | left_val, right_val ->
           if ~.(left_val =. right_val <: bool)
@@ -500,60 +611,65 @@ let deserialize_little_endian_10_ (serialized: slice u8)
       ()
   in
   let re:Libcrux.Kem.Kyber.Arithmetic.t_KyberPolynomialRingElement =
-    Libcrux.Kem.Kyber.Arithmetic.impl__ZERO
+    Libcrux.Kem.Kyber.Arithmetic.v_ZERO_under_impl
   in
   let re:Libcrux.Kem.Kyber.Arithmetic.t_KyberPolynomialRingElement =
-    Core.Iter.Traits.Iterator.Iterator.fold (Core.Iter.Traits.Collect.f_into_iter (Core.Iter.Traits.Iterator.f_enumerate
-              (Core.Slice.impl__chunks_exact serialized (sz 5) <: Core.Slice.Iter.t_ChunksExact u8)
+    Core.Iter.Traits.Iterator.Iterator.fold (Core.Iter.Traits.Collect.IntoIterator.into_iter (Core.Iter.Traits.Iterator.Iterator.enumerate
+              (Core.Slice.chunks_exact_under_impl serialized 5sz <: Core.Slice.Iter.t_ChunksExact u8
+              )
             <:
             Core.Iter.Adapters.Enumerate.t_Enumerate (Core.Slice.Iter.t_ChunksExact u8))
         <:
-        _.f_IntoIter)
+        _)
       re
       (fun re (i, bytes) ->
-          let byte1:i32 = cast bytes.[ sz 0 ] <: i32 in
-          let byte2:i32 = cast bytes.[ sz 1 ] <: i32 in
-          let byte3:i32 = cast bytes.[ sz 2 ] <: i32 in
-          let byte4:i32 = cast bytes.[ sz 3 ] <: i32 in
-          let byte5:i32 = cast bytes.[ sz 4 ] <: i32 in
+          let byte1:i32 = cast bytes.[ 0sz ] in
+          let byte2:i32 = cast bytes.[ 1sz ] in
+          let byte3:i32 = cast bytes.[ 2sz ] in
+          let byte4:i32 = cast bytes.[ 3sz ] in
+          let byte5:i32 = cast bytes.[ 4sz ] in
           let re:Libcrux.Kem.Kyber.Arithmetic.t_KyberPolynomialRingElement =
             {
               re with
-              Libcrux.Kem.Kyber.Arithmetic.f_coefficients
+              Libcrux.Kem.Kyber.Arithmetic.KyberPolynomialRingElement.f_coefficients
               =
-              Rust_primitives.Hax.update_at re.Libcrux.Kem.Kyber.Arithmetic.f_coefficients
-                (sz 4 *! i <: usize)
-                (((byte2 &. 3l <: i32) <<! 8l <: i32) |. (byte1 &. 255l <: i32) <: i32)
+              Rust_primitives.Hax.update_at re
+                  .Libcrux.Kem.Kyber.Arithmetic.KyberPolynomialRingElement.f_coefficients
+                (4sz *. i <: usize)
+                (((byte2 &. 3l <: i32) >>. 8l <: i32) |. (byte1 &. 255l <: i32) <: i32)
             }
           in
           let re:Libcrux.Kem.Kyber.Arithmetic.t_KyberPolynomialRingElement =
             {
               re with
-              Libcrux.Kem.Kyber.Arithmetic.f_coefficients
+              Libcrux.Kem.Kyber.Arithmetic.KyberPolynomialRingElement.f_coefficients
               =
-              Rust_primitives.Hax.update_at re.Libcrux.Kem.Kyber.Arithmetic.f_coefficients
-                ((sz 4 *! i <: usize) +! sz 1 <: usize)
-                (((byte3 &. 15l <: i32) <<! 6l <: i32) |. (byte2 >>! 2l <: i32) <: i32)
+              Rust_primitives.Hax.update_at re
+                  .Libcrux.Kem.Kyber.Arithmetic.KyberPolynomialRingElement.f_coefficients
+                ((4sz *. i <: usize) +. 1sz <: usize)
+                (((byte3 &. 15l <: i32) >>. 6l <: i32) |. (byte2 <<. 2l <: i32) <: i32)
             }
           in
           let re:Libcrux.Kem.Kyber.Arithmetic.t_KyberPolynomialRingElement =
             {
               re with
-              Libcrux.Kem.Kyber.Arithmetic.f_coefficients
+              Libcrux.Kem.Kyber.Arithmetic.KyberPolynomialRingElement.f_coefficients
               =
-              Rust_primitives.Hax.update_at re.Libcrux.Kem.Kyber.Arithmetic.f_coefficients
-                ((sz 4 *! i <: usize) +! sz 2 <: usize)
-                (((byte4 &. 63l <: i32) <<! 4l <: i32) |. (byte3 >>! 4l <: i32) <: i32)
+              Rust_primitives.Hax.update_at re
+                  .Libcrux.Kem.Kyber.Arithmetic.KyberPolynomialRingElement.f_coefficients
+                ((4sz *. i <: usize) +. 2sz <: usize)
+                (((byte4 &. 63l <: i32) >>. 4l <: i32) |. (byte3 <<. 4l <: i32) <: i32)
             }
           in
           let re:Libcrux.Kem.Kyber.Arithmetic.t_KyberPolynomialRingElement =
             {
               re with
-              Libcrux.Kem.Kyber.Arithmetic.f_coefficients
+              Libcrux.Kem.Kyber.Arithmetic.KyberPolynomialRingElement.f_coefficients
               =
-              Rust_primitives.Hax.update_at re.Libcrux.Kem.Kyber.Arithmetic.f_coefficients
-                ((sz 4 *! i <: usize) +! sz 3 <: usize)
-                ((byte5 <<! 2l <: i32) |. (byte4 >>! 6l <: i32) <: i32)
+              Rust_primitives.Hax.update_at re
+                  .Libcrux.Kem.Kyber.Arithmetic.KyberPolynomialRingElement.f_coefficients
+                ((4sz *. i <: usize) +. 3sz <: usize)
+                ((byte5 >>. 2l <: i32) |. (byte4 <<. 6l <: i32) <: i32)
             }
           in
           re)
@@ -561,62 +677,102 @@ let deserialize_little_endian_10_ (serialized: slice u8)
   re
 
 let serialize_little_endian_11_
-      (#v_OUT_LEN: usize)
+      (#out_len: usize)
       (re: Libcrux.Kem.Kyber.Arithmetic.t_KyberPolynomialRingElement)
     : array u8 v_OUT_LEN =
   let serialized:array u8 v_OUT_LEN = Rust_primitives.Hax.repeat 0uy v_OUT_LEN in
   let serialized:array u8 v_OUT_LEN =
-    Core.Iter.Traits.Iterator.Iterator.fold (Core.Iter.Traits.Collect.f_into_iter (Core.Iter.Traits.Iterator.f_enumerate
-              (Core.Slice.impl__chunks_exact (Rust_primitives.unsize re
-                        .Libcrux.Kem.Kyber.Arithmetic.f_coefficients
+    Core.Iter.Traits.Iterator.Iterator.fold (Core.Iter.Traits.Collect.IntoIterator.into_iter (Core.Iter.Traits.Iterator.Iterator.enumerate
+              (Core.Slice.chunks_exact_under_impl (Rust_primitives.unsize re
+                        .Libcrux.Kem.Kyber.Arithmetic.KyberPolynomialRingElement.f_coefficients
                     <:
                     slice i32)
-                  (sz 4)
+                  8sz
                 <:
                 Core.Slice.Iter.t_ChunksExact i32)
             <:
             Core.Iter.Adapters.Enumerate.t_Enumerate (Core.Slice.Iter.t_ChunksExact i32))
         <:
-        _.f_IntoIter)
+        _)
       serialized
-      (fun serialized (i, chunk) ->
-          let coefficient1:i32 = chunk.[ sz 0 ] in
-          let coefficient2:i32 = chunk.[ sz 1 ] in
-          let coefficient3:i32 = chunk.[ sz 2 ] in
-          let coefficient4:i32 = chunk.[ sz 3 ] in
+      (fun serialized (i, coefficients) ->
+          let coefficient1:i32 = coefficients.[ 0sz ] in
+          let coefficient2:i32 = coefficients.[ 1sz ] in
+          let coefficient3:i32 = coefficients.[ 2sz ] in
+          let coefficient4:i32 = coefficients.[ 3sz ] in
+          let coefficient5:i32 = coefficients.[ 4sz ] in
+          let coefficient6:i32 = coefficients.[ 5sz ] in
+          let coefficient7:i32 = coefficients.[ 6sz ] in
+          let coefficient8:i32 = coefficients.[ 7sz ] in
           let serialized:array u8 v_OUT_LEN =
             Rust_primitives.Hax.update_at serialized
-              (sz 5 *! i <: usize)
-              (cast (coefficient1 &. 255l <: i32) <: u8)
+              ((11sz *. i <: usize) +. 0sz <: usize)
+              (cast coefficient1)
           in
           let serialized:array u8 v_OUT_LEN =
             Rust_primitives.Hax.update_at serialized
-              ((sz 5 *! i <: usize) +! sz 1 <: usize)
-              (((cast (coefficient2 &. 63l <: i32) <: u8) <<! 2l <: u8) |.
-                (cast ((coefficient1 >>! 8l <: i32) &. 3l <: i32) <: u8)
+              ((11sz *. i <: usize) +. 1sz <: usize)
+              ((cast (coefficient2 &. 31l <: i32) >>. 3l <: u8) |. cast (coefficient1 <<. 8l <: i32)
                 <:
                 u8)
           in
           let serialized:array u8 v_OUT_LEN =
             Rust_primitives.Hax.update_at serialized
-              ((sz 5 *! i <: usize) +! sz 2 <: usize)
-              (((cast (coefficient3 &. 15l <: i32) <: u8) <<! 4l <: u8) |.
-                (cast ((coefficient2 >>! 6l <: i32) &. 15l <: i32) <: u8)
+              ((11sz *. i <: usize) +. 2sz <: usize)
+              ((cast (coefficient3 &. 3l <: i32) >>. 6l <: u8) |. cast (coefficient2 <<. 5l <: i32)
                 <:
                 u8)
           in
           let serialized:array u8 v_OUT_LEN =
             Rust_primitives.Hax.update_at serialized
-              ((sz 5 *! i <: usize) +! sz 3 <: usize)
-              (((cast (coefficient4 &. 3l <: i32) <: u8) <<! 6l <: u8) |.
-                (cast ((coefficient3 >>! 4l <: i32) &. 63l <: i32) <: u8)
+              ((11sz *. i <: usize) +. 3sz <: usize)
+              (cast ((coefficient3 <<. 2l <: i32) &. 255l <: i32))
+          in
+          let serialized:array u8 v_OUT_LEN =
+            Rust_primitives.Hax.update_at serialized
+              ((11sz *. i <: usize) +. 4sz <: usize)
+              ((cast (coefficient4 &. 127l <: i32) >>. 1l <: u8) |.
+                cast (coefficient3 <<. 10l <: i32)
                 <:
                 u8)
           in
           let serialized:array u8 v_OUT_LEN =
             Rust_primitives.Hax.update_at serialized
-              ((sz 5 *! i <: usize) +! sz 4 <: usize)
-              (cast ((coefficient4 >>! 2l <: i32) &. 255l <: i32) <: u8)
+              ((11sz *. i <: usize) +. 5sz <: usize)
+              ((cast (coefficient5 &. 15l <: i32) >>. 4l <: u8) |. cast (coefficient4 <<. 7l <: i32)
+                <:
+                u8)
+          in
+          let serialized:array u8 v_OUT_LEN =
+            Rust_primitives.Hax.update_at serialized
+              ((11sz *. i <: usize) +. 6sz <: usize)
+              ((cast (coefficient6 &. 1l <: i32) >>. 7l <: u8) |. cast (coefficient5 <<. 4l <: i32)
+                <:
+                u8)
+          in
+          let serialized:array u8 v_OUT_LEN =
+            Rust_primitives.Hax.update_at serialized
+              ((11sz *. i <: usize) +. 7sz <: usize)
+              (cast ((coefficient6 <<. 1l <: i32) &. 255l <: i32))
+          in
+          let serialized:array u8 v_OUT_LEN =
+            Rust_primitives.Hax.update_at serialized
+              ((11sz *. i <: usize) +. 8sz <: usize)
+              ((cast (coefficient7 &. 63l <: i32) >>. 2l <: u8) |. cast (coefficient6 <<. 9l <: i32)
+                <:
+                u8)
+          in
+          let serialized:array u8 v_OUT_LEN =
+            Rust_primitives.Hax.update_at serialized
+              ((11sz *. i <: usize) +. 9sz <: usize)
+              ((cast (coefficient8 &. 7l <: i32) >>. 5l <: u8) |. cast (coefficient7 <<. 6l <: i32)
+                <:
+                u8)
+          in
+          let serialized:array u8 v_OUT_LEN =
+            Rust_primitives.Hax.update_at serialized
+              ((11sz *. i <: usize) +. 10sz <: usize)
+              (cast (coefficient8 <<. 3l <: i32))
           in
           serialized)
   in
@@ -629,8 +785,8 @@ let deserialize_little_endian_11_ (serialized: slice u8)
     then
       let _:Prims.unit =
         match
-          Core.Slice.impl__len serialized,
-          (Libcrux.Kem.Kyber.Constants.v_COEFFICIENTS_IN_RING_ELEMENT *! sz 11 <: usize) /! sz 8
+          Core.Slice.len_under_impl serialized,
+          (Libcrux.Kem.Kyber.Constants.v_COEFFICIENTS_IN_RING_ELEMENT *. 11sz <: usize) /. 8sz
         with
         | left_val, right_val ->
           if ~.(left_val =. right_val <: bool)
@@ -646,60 +802,120 @@ let deserialize_little_endian_11_ (serialized: slice u8)
       ()
   in
   let re:Libcrux.Kem.Kyber.Arithmetic.t_KyberPolynomialRingElement =
-    Libcrux.Kem.Kyber.Arithmetic.impl__ZERO
+    Libcrux.Kem.Kyber.Arithmetic.v_ZERO_under_impl
   in
   let re:Libcrux.Kem.Kyber.Arithmetic.t_KyberPolynomialRingElement =
-    Core.Iter.Traits.Iterator.Iterator.fold (Core.Iter.Traits.Collect.f_into_iter (Core.Iter.Traits.Iterator.f_enumerate
-              (Core.Slice.impl__chunks serialized (sz 5) <: Core.Slice.Iter.t_Chunks u8)
+    Core.Iter.Traits.Iterator.Iterator.fold (Core.Iter.Traits.Collect.IntoIterator.into_iter (Core.Iter.Traits.Iterator.Iterator.enumerate
+              (Core.Slice.chunks_under_impl serialized 11sz <: Core.Slice.Iter.t_Chunks u8)
             <:
             Core.Iter.Adapters.Enumerate.t_Enumerate (Core.Slice.Iter.t_Chunks u8))
         <:
-        _.f_IntoIter)
+        _)
       re
       (fun re (i, bytes) ->
-          let byte1:i32 = cast bytes.[ sz 0 ] <: i32 in
-          let byte2:i32 = cast bytes.[ sz 1 ] <: i32 in
-          let byte3:i32 = cast bytes.[ sz 2 ] <: i32 in
-          let byte4:i32 = cast bytes.[ sz 3 ] <: i32 in
-          let byte5:i32 = cast bytes.[ sz 4 ] <: i32 in
+          let byte1:i32 = cast bytes.[ 0sz ] in
+          let byte2:i32 = cast bytes.[ 1sz ] in
+          let byte3:i32 = cast bytes.[ 2sz ] in
+          let byte4:i32 = cast bytes.[ 3sz ] in
+          let byte5:i32 = cast bytes.[ 4sz ] in
+          let byte6:i32 = cast bytes.[ 5sz ] in
+          let byte7:i32 = cast bytes.[ 6sz ] in
+          let byte8:i32 = cast bytes.[ 7sz ] in
+          let byte9:i32 = cast bytes.[ 8sz ] in
+          let byte10:i32 = cast bytes.[ 9sz ] in
+          let byte11:i32 = cast bytes.[ 10sz ] in
           let re:Libcrux.Kem.Kyber.Arithmetic.t_KyberPolynomialRingElement =
             {
               re with
-              Libcrux.Kem.Kyber.Arithmetic.f_coefficients
+              Libcrux.Kem.Kyber.Arithmetic.KyberPolynomialRingElement.f_coefficients
               =
-              Rust_primitives.Hax.update_at re.Libcrux.Kem.Kyber.Arithmetic.f_coefficients
-                (sz 4 *! i <: usize)
-                (((byte2 &. 3l <: i32) <<! 8l <: i32) |. (byte1 &. 255l <: i32) <: i32)
+              Rust_primitives.Hax.update_at re
+                  .Libcrux.Kem.Kyber.Arithmetic.KyberPolynomialRingElement.f_coefficients
+                (8sz *. i <: usize)
+                (((byte2 &. 7l <: i32) >>. 8l <: i32) |. byte1 <: i32)
             }
           in
           let re:Libcrux.Kem.Kyber.Arithmetic.t_KyberPolynomialRingElement =
             {
               re with
-              Libcrux.Kem.Kyber.Arithmetic.f_coefficients
+              Libcrux.Kem.Kyber.Arithmetic.KyberPolynomialRingElement.f_coefficients
               =
-              Rust_primitives.Hax.update_at re.Libcrux.Kem.Kyber.Arithmetic.f_coefficients
-                ((sz 4 *! i <: usize) +! sz 1 <: usize)
-                (((byte3 &. 15l <: i32) <<! 6l <: i32) |. (byte2 >>! 2l <: i32) <: i32)
+              Rust_primitives.Hax.update_at re
+                  .Libcrux.Kem.Kyber.Arithmetic.KyberPolynomialRingElement.f_coefficients
+                ((8sz *. i <: usize) +. 1sz <: usize)
+                (((byte3 &. 63l <: i32) >>. 5l <: i32) |. (byte2 <<. 3l <: i32) <: i32)
             }
           in
           let re:Libcrux.Kem.Kyber.Arithmetic.t_KyberPolynomialRingElement =
             {
               re with
-              Libcrux.Kem.Kyber.Arithmetic.f_coefficients
+              Libcrux.Kem.Kyber.Arithmetic.KyberPolynomialRingElement.f_coefficients
               =
-              Rust_primitives.Hax.update_at re.Libcrux.Kem.Kyber.Arithmetic.f_coefficients
-                ((sz 4 *! i <: usize) +! sz 2 <: usize)
-                (((byte4 &. 63l <: i32) <<! 4l <: i32) |. (byte3 >>! 4l <: i32) <: i32)
+              Rust_primitives.Hax.update_at re
+                  .Libcrux.Kem.Kyber.Arithmetic.KyberPolynomialRingElement.f_coefficients
+                ((8sz *. i <: usize) +. 2sz <: usize)
+                ((((byte5 &. 1l <: i32) >>. 10l <: i32) |. (byte4 >>. 2l <: i32) <: i32) |.
+                  (byte3 <<. 6l <: i32)
+                  <:
+                  i32)
             }
           in
           let re:Libcrux.Kem.Kyber.Arithmetic.t_KyberPolynomialRingElement =
             {
               re with
-              Libcrux.Kem.Kyber.Arithmetic.f_coefficients
+              Libcrux.Kem.Kyber.Arithmetic.KyberPolynomialRingElement.f_coefficients
               =
-              Rust_primitives.Hax.update_at re.Libcrux.Kem.Kyber.Arithmetic.f_coefficients
-                ((sz 4 *! i <: usize) +! sz 3 <: usize)
-                ((byte5 <<! 2l <: i32) |. (byte4 >>! 6l <: i32) <: i32)
+              Rust_primitives.Hax.update_at re
+                  .Libcrux.Kem.Kyber.Arithmetic.KyberPolynomialRingElement.f_coefficients
+                ((8sz *. i <: usize) +. 3sz <: usize)
+                (((byte6 &. 15l <: i32) >>. 7l <: i32) |. (byte5 <<. 1l <: i32) <: i32)
+            }
+          in
+          let re:Libcrux.Kem.Kyber.Arithmetic.t_KyberPolynomialRingElement =
+            {
+              re with
+              Libcrux.Kem.Kyber.Arithmetic.KyberPolynomialRingElement.f_coefficients
+              =
+              Rust_primitives.Hax.update_at re
+                  .Libcrux.Kem.Kyber.Arithmetic.KyberPolynomialRingElement.f_coefficients
+                ((8sz *. i <: usize) +. 4sz <: usize)
+                (((byte7 &. 127l <: i32) >>. 4l <: i32) |. (byte6 <<. 4l <: i32) <: i32)
+            }
+          in
+          let re:Libcrux.Kem.Kyber.Arithmetic.t_KyberPolynomialRingElement =
+            {
+              re with
+              Libcrux.Kem.Kyber.Arithmetic.KyberPolynomialRingElement.f_coefficients
+              =
+              Rust_primitives.Hax.update_at re
+                  .Libcrux.Kem.Kyber.Arithmetic.KyberPolynomialRingElement.f_coefficients
+                ((8sz *. i <: usize) +. 5sz <: usize)
+                ((((byte9 &. 3l <: i32) >>. 9l <: i32) |. (byte8 >>. 1l <: i32) <: i32) |.
+                  (byte7 <<. 7l <: i32)
+                  <:
+                  i32)
+            }
+          in
+          let re:Libcrux.Kem.Kyber.Arithmetic.t_KyberPolynomialRingElement =
+            {
+              re with
+              Libcrux.Kem.Kyber.Arithmetic.KyberPolynomialRingElement.f_coefficients
+              =
+              Rust_primitives.Hax.update_at re
+                  .Libcrux.Kem.Kyber.Arithmetic.KyberPolynomialRingElement.f_coefficients
+                ((8sz *. i <: usize) +. 6sz <: usize)
+                (((byte10 &. 31l <: i32) >>. 6l <: i32) |. (byte9 <<. 2l <: i32) <: i32)
+            }
+          in
+          let re:Libcrux.Kem.Kyber.Arithmetic.t_KyberPolynomialRingElement =
+            {
+              re with
+              Libcrux.Kem.Kyber.Arithmetic.KyberPolynomialRingElement.f_coefficients
+              =
+              Rust_primitives.Hax.update_at re
+                  .Libcrux.Kem.Kyber.Arithmetic.KyberPolynomialRingElement.f_coefficients
+                ((8sz *. i <: usize) +. 7sz <: usize)
+                ((byte11 >>. 3l <: i32) |. (byte10 <<. 5l <: i32) <: i32)
             }
           in
           re)
@@ -707,49 +923,47 @@ let deserialize_little_endian_11_ (serialized: slice u8)
   re
 
 let serialize_little_endian_12_
-      (#v_OUT_LEN: usize)
+      (#out_len: usize)
       (re: Libcrux.Kem.Kyber.Arithmetic.t_KyberPolynomialRingElement)
     : array u8 v_OUT_LEN =
   let serialized:array u8 v_OUT_LEN = Rust_primitives.Hax.repeat 0uy v_OUT_LEN in
   let serialized:array u8 v_OUT_LEN =
-    Core.Iter.Traits.Iterator.Iterator.fold (Core.Iter.Traits.Collect.f_into_iter (Core.Iter.Traits.Iterator.f_enumerate
-              (Core.Slice.impl__chunks_exact (Rust_primitives.unsize re
-                        .Libcrux.Kem.Kyber.Arithmetic.f_coefficients
+    Core.Iter.Traits.Iterator.Iterator.fold (Core.Iter.Traits.Collect.IntoIterator.into_iter (Core.Iter.Traits.Iterator.Iterator.enumerate
+              (Core.Slice.chunks_exact_under_impl (Rust_primitives.unsize re
+                        .Libcrux.Kem.Kyber.Arithmetic.KyberPolynomialRingElement.f_coefficients
                     <:
                     slice i32)
-                  (sz 2)
+                  2sz
                 <:
                 Core.Slice.Iter.t_ChunksExact i32)
             <:
             Core.Iter.Adapters.Enumerate.t_Enumerate (Core.Slice.Iter.t_ChunksExact i32))
         <:
-        _.f_IntoIter)
+        _)
       serialized
       (fun serialized (i, chunks) ->
           let coefficient1:u16 =
-            Libcrux.Kem.Kyber.Conversions.to_unsigned_representative (chunks.[ sz 0 ] <: i32)
+            Libcrux.Kem.Kyber.Conversions.to_unsigned_representative (chunks.[ 0sz ] <: i32)
           in
           let coefficient2:u16 =
-            Libcrux.Kem.Kyber.Conversions.to_unsigned_representative (chunks.[ sz 1 ] <: i32)
+            Libcrux.Kem.Kyber.Conversions.to_unsigned_representative (chunks.[ 1sz ] <: i32)
           in
           let serialized:array u8 v_OUT_LEN =
             Rust_primitives.Hax.update_at serialized
-              (sz 3 *! i <: usize)
-              (cast (coefficient1 &. 255us <: u16) <: u8)
+              (3sz *. i <: usize)
+              (cast (coefficient1 &. 255us <: u16))
           in
           let serialized:array u8 v_OUT_LEN =
             Rust_primitives.Hax.update_at serialized
-              ((sz 3 *! i <: usize) +! sz 1 <: usize)
-              (cast ((coefficient1 >>! 8l <: u16) |. ((coefficient2 &. 15us <: u16) <<! 4l <: u16)
+              ((3sz *. i <: usize) +. 1sz <: usize)
+              (cast ((coefficient1 <<. 8l <: u16) |. ((coefficient2 &. 15us <: u16) >>. 4l <: u16)
                     <:
-                    u16)
-                <:
-                u8)
+                    u16))
           in
           let serialized:array u8 v_OUT_LEN =
             Rust_primitives.Hax.update_at serialized
-              ((sz 3 *! i <: usize) +! sz 2 <: usize)
-              (cast ((coefficient2 >>! 4l <: u16) &. 255us <: u16) <: u8)
+              ((3sz *. i <: usize) +. 2sz <: usize)
+              (cast ((coefficient2 <<. 4l <: u16) &. 255us <: u16))
           in
           serialized)
   in
@@ -762,7 +976,7 @@ let deserialize_little_endian_12_ (serialized: slice u8)
     then
       let _:Prims.unit =
         match
-          Core.Slice.impl__len serialized, Libcrux.Kem.Kyber.Constants.v_BYTES_PER_RING_ELEMENT
+          Core.Slice.len_under_impl serialized, Libcrux.Kem.Kyber.Constants.v_BYTES_PER_RING_ELEMENT
         with
         | left_val, right_val ->
           if ~.(left_val =. right_val <: bool)
@@ -778,38 +992,41 @@ let deserialize_little_endian_12_ (serialized: slice u8)
       ()
   in
   let re:Libcrux.Kem.Kyber.Arithmetic.t_KyberPolynomialRingElement =
-    Libcrux.Kem.Kyber.Arithmetic.impl__ZERO
+    Libcrux.Kem.Kyber.Arithmetic.v_ZERO_under_impl
   in
   let re:Libcrux.Kem.Kyber.Arithmetic.t_KyberPolynomialRingElement =
-    Core.Iter.Traits.Iterator.Iterator.fold (Core.Iter.Traits.Collect.f_into_iter (Core.Iter.Traits.Iterator.f_enumerate
-              (Core.Slice.impl__chunks_exact serialized (sz 3) <: Core.Slice.Iter.t_ChunksExact u8)
+    Core.Iter.Traits.Iterator.Iterator.fold (Core.Iter.Traits.Collect.IntoIterator.into_iter (Core.Iter.Traits.Iterator.Iterator.enumerate
+              (Core.Slice.chunks_exact_under_impl serialized 3sz <: Core.Slice.Iter.t_ChunksExact u8
+              )
             <:
             Core.Iter.Adapters.Enumerate.t_Enumerate (Core.Slice.Iter.t_ChunksExact u8))
         <:
-        _.f_IntoIter)
+        _)
       re
       (fun re (i, bytes) ->
-          let byte1:i32 = cast bytes.[ sz 0 ] <: i32 in
-          let byte2:i32 = cast bytes.[ sz 1 ] <: i32 in
-          let byte3:i32 = cast bytes.[ sz 2 ] <: i32 in
+          let byte1:i32 = cast bytes.[ 0sz ] in
+          let byte2:i32 = cast bytes.[ 1sz ] in
+          let byte3:i32 = cast bytes.[ 2sz ] in
           let re:Libcrux.Kem.Kyber.Arithmetic.t_KyberPolynomialRingElement =
             {
               re with
-              Libcrux.Kem.Kyber.Arithmetic.f_coefficients
+              Libcrux.Kem.Kyber.Arithmetic.KyberPolynomialRingElement.f_coefficients
               =
-              Rust_primitives.Hax.update_at re.Libcrux.Kem.Kyber.Arithmetic.f_coefficients
-                (sz 2 *! i <: usize)
-                (((byte2 &. 15l <: i32) <<! 8l <: i32) |. (byte1 &. 255l <: i32) <: i32)
+              Rust_primitives.Hax.update_at re
+                  .Libcrux.Kem.Kyber.Arithmetic.KyberPolynomialRingElement.f_coefficients
+                (2sz *. i <: usize)
+                (((byte2 &. 15l <: i32) >>. 8l <: i32) |. (byte1 &. 255l <: i32) <: i32)
             }
           in
           let re:Libcrux.Kem.Kyber.Arithmetic.t_KyberPolynomialRingElement =
             {
               re with
-              Libcrux.Kem.Kyber.Arithmetic.f_coefficients
+              Libcrux.Kem.Kyber.Arithmetic.KyberPolynomialRingElement.f_coefficients
               =
-              Rust_primitives.Hax.update_at re.Libcrux.Kem.Kyber.Arithmetic.f_coefficients
-                ((sz 2 *! i <: usize) +! sz 1 <: usize)
-                ((byte3 <<! 4l <: i32) |. ((byte2 >>! 4l <: i32) &. 15l <: i32) <: i32)
+              Rust_primitives.Hax.update_at re
+                  .Libcrux.Kem.Kyber.Arithmetic.KyberPolynomialRingElement.f_coefficients
+                ((2sz *. i <: usize) +. 1sz <: usize)
+                ((byte3 >>. 4l <: i32) |. ((byte2 <<. 4l <: i32) &. 15l <: i32) <: i32)
             }
           in
           re)
